handle reduction flags in reduction and conversion

theories/MetaTheory/Conversion/ContextConversion.v
@@ -8,62 +8,89 @@ From Metaprog.MetaTheory Require Export Conversion.SubstConversion.
 (** * Conversion relation on contexts. *)
 (***********************************************************************)
 
-(** [cconv Σ Γ Γ'] means that contexts [Γ] and [Γ'] are convertible
+(** [cconv flags Σ Γ Γ'] means that contexts [Γ] and [Γ'] are convertible
     in evar-map [Σ]. *)
-Inductive cconv (Σ : evar_map) : forall {s}, context ∅ s -> context ∅ s -> Prop :=
-| cconv_nil : cconv Σ CNil CNil
+Inductive cconv (flags : red_flags) (Σ : evar_map) : forall {s}, context ∅ s -> context ∅ s -> Prop :=
+| cconv_nil : cconv flags Σ CNil CNil
 
 | cconv_cons {s} x (ty ty' : term s) Γ Γ' :
-    Σ ⊢ ty ≡ ty' ->
-    cconv Σ Γ Γ' ->
-    cconv Σ (CCons Γ x ty) (CCons Γ' x ty').
+    Σ ⊢ ty ≡{flags} ty' ->
+    cconv flags Σ Γ Γ' ->
+    cconv flags Σ (CCons Γ x ty) (CCons Γ' x ty').
 
 Derive Signature for cconv.
 
-#[export] Instance cconv_Reflexive Σ s : Reflexive (@cconv Σ s).
+(***********************************************************************)
+(** * Typeclass instances for setoid rewriting. *)
+(***********************************************************************)
+
+Section Instances.
+  Context {flags : red_flags} {Σ : evar_map}.
+
+  #[export] Instance cconv_Reflexive s : Reflexive (@cconv flags Σ s).
+  Proof.
+  intros Γ. induction Γ ; constructor.
+  - reflexivity.
+  - assumption.
+  Qed.
+
+  #[export] Instance cconv_Symmetric s : Symmetric (@cconv flags Σ s).
+  Proof.
+  intros Γ Γ' HΓ. induction HΓ ; constructor.
+  - now symmetry.
+  - assumption.
+  Qed.
+
+  #[export] Instance cconv_Transitive s : Transitive (@cconv flags Σ s).
+  Proof.
+  intros Γ1 Γ2 Γ3 H1 H2. induction H1 ; depelim H2.
+  - reflexivity.
+  - constructor.
+    + now rewrite H.
+    + now apply IHcconv.
+  Qed.
+
+  #[export] Instance cconv_of_cred1 s : subrelation (@cred1 flags Σ s) (@cconv flags Σ s).
+  Proof.
+  intros Γ Γ' HΓ. induction HΓ ; constructor.
+  - now rewrite H.
+  - reflexivity.
+  - reflexivity.
+  - assumption.
+  Qed.
+
+  #[export] Instance cconv_of_cred s : subrelation (@cred flags Σ s) (@cconv flags Σ s).
+  Proof.
+  intros Γ Γ' HΓ. induction HΓ ; constructor.
+  - now rewrite H.
+  - assumption.
+  Qed.
+
+End Instances.
+
+Lemma cconv_extend_flags {flags1 flags2 Σ s} :
+  red_flags_incl flags1 flags2 ->
+  subrelation (@cconv flags1 Σ s) (@cconv flags2 Σ s).
 Proof.
-intros Γ. induction Γ ; constructor.
-- reflexivity.
+intros Hf Γ Γ' HΓ. induction HΓ ; constructor.
+- now apply (conv_extend_flags Hf).
 - assumption.
 Qed.
 
-#[export] Instance cconv_Symmetric Σ s : Symmetric (@cconv Σ s).
-Proof.
-intros Γ Γ' HΓ. induction HΓ ; constructor.
-- now symmetry.
-- assumption.
-Qed.
+(***********************************************************************)
+(** * Lemmas about context conversion. *)
+(***********************************************************************)
 
-#[export] Instance cconv_Transitive Σ s : Transitive (@cconv Σ s).
-Proof.
-intros Γ1 Γ2 Γ3 H1 H2. induction H1 ; depelim H2.
-- reflexivity.
-- constructor.
-  + now rewrite H.
-  + now apply IHcconv.
-Qed.
+Section Lemmas.
+  Context {flags : red_flags} {Σ : evar_map}.
 
-#[export] Instance cconv_of_cred1 Σ s : subrelation (@cred1 Σ s) (@cconv Σ s).
-Proof.
-intros Γ Γ' HΓ. induction HΓ ; constructor.
-- now rewrite H.
-- reflexivity.
-- reflexivity.
-- assumption.
-Qed.
+  Lemma lookup_context_cconv {s} (i : index s) Γ Γ' :
+    cconv flags Σ Γ Γ' ->
+    Σ ⊢ lookup_context i Γ ≡{flags} lookup_context i Γ'.
+  Proof.
+  intros H. induction H ; depelim i ; simp lookup_context ; simpl_subst.
+  - now rewrite H.
+  - now rewrite IHcconv.
+  Qed.
 
-#[export] Instance cconv_of_cred Σ s : subrelation (@cred Σ s) (@cconv Σ s).
-Proof.
-intros Γ Γ' HΓ. induction HΓ ; constructor.
-- now rewrite H.
-- assumption.
-Qed.
-
-Lemma lookup_context_cconv {s Σ} (i : index s) Γ Γ' :
-  cconv Σ Γ Γ' ->
-  Σ ⊢ lookup_context i Γ ≡ lookup_context i Γ'.
-Proof.
-intros H. induction H ; depelim i ; simp lookup_context ; simpl_subst.
-- now rewrite H.
-- now rewrite IHcconv.
-Qed.
+End Lemmas.
