theories/MetaTheory/Conversion/SubstConversion.v
@@ -12,32 +12,49 @@ From Metaprog.MetaTheory Require Export Conversion.TermConversion.
 
 (** Conversion on substitutions is just pointwise conversion.
     We wrap the definition in a record to avoid setoid rewrite issues. *)
-Record sconv {s s'} (Σ : evar_map) (σ σ' : subst s s') : Prop := {
-  sconv_prop : forall i, Σ ⊢ sapply σ i ≡ sapply σ' i
+Record sconv (flags : red_flags) (Σ : evar_map) {s s'} (σ σ' : subst s s') : Prop := {
+  sconv_prop : forall i, Σ ⊢ sapply σ i ≡{flags} sapply σ' i
 }.
 
-#[export] Instance sconv_Reflexive s s' Σ : Reflexive (@sconv s s' Σ).
-Proof. intros σ. constructor. reflexivity. Qed.
-
-#[export] Instance sconv_Symmetric s s' Σ : Symmetric (@sconv s s' Σ).
-Proof. intros σ σ' [Hσ]. constructor. intros i. now symmetry. Qed.
-
-#[export] Instance sconv_Transitive s s' Σ : Transitive (@sconv s s' Σ).
-Proof.
-intros σ1 σ2 σ3 [H1] [H2]. constructor. intros i. etransitivity ; eauto.
-Qed.
-
-#[export] Instance conv_sapply {s s'} Σ :
-  Proper (sconv Σ ==> eq ==> conv Σ) (@sapply s s').
+#[export] Instance conv_sapply flags Σ s s' :
+  Proper (sconv flags Σ ==> eq ==> conv flags Σ) (@sapply s s').
 Proof. intros σ σ' [Hσ] i ? <-. apply Hσ. Qed.
 
-#[export] Instance sconv_of_sred {s s'} Σ :
-  subrelation (@sred s s' Σ) (@sconv s s' Σ).
-Proof. intros σ σ' Hσ. constructor. intros i. now rewrite Hσ. Qed.
+(***********************************************************************)
+(** * Typeclass instances for setoid rewriting. *)
+(***********************************************************************)
 
-#[export] Instance sconv_of_sred_flip {s s'} Σ :
-  subrelation (Basics.flip (@sred s s' Σ)) (@sconv s s' Σ).
-Proof. intros σ σ' Hσ. constructor. intros i. now rewrite Hσ. Qed.
+Section Instances.
+  Context {flags : red_flags} {Σ : evar_map} {s s' : scope}.
+
+  #[export] Instance sconv_Reflexive : Reflexive (@sconv flags Σ s s').
+  Proof. intros σ. constructor. reflexivity. Qed.
+
+  #[export] Instance sconv_Symmetric : Symmetric (@sconv flags Σ s s').
+  Proof. intros σ σ' [Hσ]. constructor. intros i. now symmetry. Qed.
+
+  #[export] Instance sconv_Transitive : Transitive (@sconv flags Σ s s').
+  Proof.
+  intros σ1 σ2 σ3 [H1] [H2]. constructor. intros i. etransitivity ; eauto.
+  Qed.
+
+  #[export] Instance sconv_of_sred :
+    subrelation (@sred flags Σ s s') (@sconv flags Σ s s').
+  Proof. intros σ σ' Hσ. constructor. intros i. now rewrite Hσ. Qed.
+
+  #[export] Instance sconv_of_sred_flip :
+    subrelation (Basics.flip (@sred flags Σ s s')) (@sconv flags Σ s s').
+  Proof. intros σ σ' Hσ. constructor. intros i. now rewrite Hσ. Qed.
+
+End Instances.
+
+Lemma sconv_extend_flags {flags1 flags2 Σ s s'} :
+  red_flags_incl flags1 flags2 ->
+  subrelation (@sconv flags1 Σ s s') (@sconv flags2 Σ s s').
+Proof.
+intros Hf σ1 σ2 Hσ. constructor. intros i. apply (conv_extend_flags Hf).
+apply Hσ.
+Qed.
 
 (***********************************************************************)
 (** * Church-Rosser lemma. *)
@@ -45,9 +62,9 @@ Proof. intros σ σ' Hσ. constructor. intros i. now rewrite Hσ. Qed.
 
 (** Church-Rosser lemma on substitutions.
     This is a simple consequence of the Church-Rosser lemma on terms. *)
-Lemma church_rosser_subst {s s' Σ} (σ σ' : subst s s') :
-  sconv Σ σ σ' ->
-  exists τ, sred Σ σ τ /\ sred Σ σ' τ.
+Lemma church_rosser_subst {flags Σ s s'} (σ σ' : subst s s') :
+  sconv flags Σ σ σ' ->
+  exists τ, sred flags Σ σ τ /\ sred flags Σ σ' τ.
 Proof.
 revert s' σ σ'. induction s.
 - intros s' σ σ' Hσ. exists (sren wk_idx). split ; constructor ; intros i ; depelim i.
@@ -55,7 +72,7 @@ revert s' σ σ'. induction s.
   specialize (IHs s' (rscomp rshift σ) (rscomp rshift σ')).
   forward IHs. { constructor. intros i. simpl_subst. now rewrite Hσ. }
   destruct IHs as (τ & H1 & H2).
-  assert (exists t, Σ ⊢ sapply σ I0 ~~> t /\ Σ ⊢ sapply σ' I0 ~~> t) as (t & Ht1 & Ht2).
+  assert (exists t, Σ ⊢ sapply σ I0 ~~>{flags} t /\ Σ ⊢ sapply σ' I0 ~~>{flags} t) as (t & Ht1 & Ht2).
   { apply church_rosser. now rewrite Hσ. }
   exists (scons x t τ). split.
   + constructor. intros i. depelim i ; simpl_subst.
@@ -70,59 +87,64 @@ Qed.
 (** * Compatibility of conversion with renaming and substitution. *)
 (***********************************************************************)
 
-#[export] Instance conv_rename {s s' Σ} (ρ : ren s s') :
-  Proper (conv Σ ==> conv Σ) (rename ρ).
-Proof.
-intros t t' H. apply church_rosser in H. destruct H as (u & H1 & H2).
-now rewrite H1, H2.
-Qed.
+Section Substitutivity.
+  Context {flags : red_flags} {Σ : evar_map} {s s' s'' : scope} {x : tag}.
 
-#[export] Instance conv_substitute {s s' Σ} :
-  Proper (sconv Σ ==> conv Σ ==> conv Σ) (@substitute s s').
-Proof.
-intros σ σ' Hσ t t' Ht.
-apply church_rosser in Ht. destruct Ht as (u & -> & ->).
-apply church_rosser_subst in Hσ. destruct Hσ as (? & -> & ->).
-reflexivity.
-Qed.
+  #[export] Instance conv_rename (ρ : ren s s') :
+    Proper (conv flags Σ ==> conv flags Σ) (rename ρ).
+  Proof.
+  intros t t' H. apply church_rosser in H. destruct H as (u & H1 & H2).
+  now rewrite H1, H2.
+  Qed.
 
-#[export] Instance conv_scons {s s' x Σ} :
-  Proper (conv Σ ==> sconv Σ ==> sconv Σ) (@scons s s' x).
-Proof.
-intros t t' Ht σ σ' Hσ. constructor. intros i.
-apply church_rosser in Ht. destruct Ht as (? & -> & ->).
-apply church_rosser_subst in Hσ. destruct Hσ as (? & -> & ->).
-reflexivity.
-Qed.
+  #[export] Instance conv_substitute :
+    Proper (sconv flags Σ ==> conv flags Σ ==> conv flags Σ) (@substitute s s').
+  Proof.
+  intros σ σ' Hσ t t' Ht.
+  apply church_rosser in Ht. destruct Ht as (u & -> & ->).
+  apply church_rosser_subst in Hσ. destruct Hσ as (? & -> & ->).
+  reflexivity.
+  Qed.
 
-#[export] Instance conv_srcomp {s s' x Σ} :
-  Proper (sconv Σ ==> eq ==> sconv Σ) (@srcomp s s' x).
-Proof.
-intros σ σ' Hσ ρ ρ' <-. constructor. intros i.
-apply church_rosser_subst in Hσ. destruct Hσ as (? & -> & ->).
-reflexivity.
-Qed.
+  #[export] Instance conv_scons :
+    Proper (conv flags Σ ==> sconv flags Σ ==> sconv flags Σ) (@scons s s' x).
+  Proof.
+  intros t t' Ht σ σ' Hσ. constructor. intros i.
+  apply church_rosser in Ht. destruct Ht as (? & -> & ->).
+  apply church_rosser_subst in Hσ. destruct Hσ as (? & -> & ->).
+  reflexivity.
+  Qed.
 
-#[export] Instance conv_rscomp {s s' x Σ} :
-  Proper (eq ==> sconv Σ ==> sconv Σ) (@rscomp s s' x).
-Proof.
-intros ρ ρ' <- σ σ' Hσ. constructor. intros i.
-apply church_rosser_subst in Hσ. destruct Hσ as (? & -> & ->).
-reflexivity.
-Qed.
+  #[export] Instance conv_srcomp :
+    Proper (sconv flags Σ ==> eq ==> sconv flags Σ) (@srcomp s s' s'').
+  Proof.
+  intros σ σ' Hσ ρ ρ' <-. constructor. intros i.
+  apply church_rosser_subst in Hσ. destruct Hσ as (? & -> & ->).
+  reflexivity.
+  Qed.
 
-#[export] Instance conv_sup {s s' x Σ} :
-  Proper (sconv Σ ==> sconv Σ) (@sup s s' x).
-Proof.
-intros σ σ' Hσ. apply church_rosser_subst in Hσ.
-destruct Hσ as (? & -> & ->). reflexivity.
-Qed.
+  #[export] Instance conv_rscomp :
+    Proper (eq ==> sconv flags Σ ==> sconv flags Σ) (@rscomp s s' s'').
+  Proof.
+  intros ρ ρ' <- σ σ' Hσ. constructor. intros i.
+  apply church_rosser_subst in Hσ. destruct Hσ as (? & -> & ->).
+  reflexivity.
+  Qed.
 
-#[export] Instance conv_scomp {s s' x Σ} :
-  Proper (sconv Σ ==> sconv Σ ==> sconv Σ) (@scomp s s' x).
-Proof.
-intros σ σ' Hσ τ τ' Hτ. apply church_rosser_subst in Hσ, Hτ.
-destruct Hσ as (? & -> & ->). destruct Hτ as (? & -> & ->).
-reflexivity.
-Qed.
+  #[export] Instance conv_sup :
+    Proper (sconv flags Σ ==> sconv flags Σ) (@sup s s' x).
+  Proof.
+  intros σ σ' Hσ. apply church_rosser_subst in Hσ.
+  destruct Hσ as (? & -> & ->). reflexivity.
+  Qed.
+
+  #[export] Instance conv_scomp :
+    Proper (sconv flags Σ ==> sconv flags Σ ==> sconv flags Σ) (@scomp s s' s'').
+  Proof.
+  intros σ σ' Hσ τ τ' Hτ. apply church_rosser_subst in Hσ, Hτ.
+  destruct Hσ as (? & -> & ->). destruct Hτ as (? & -> & ->).
+  reflexivity.
+  Qed.
+
+End Substitutivity.
 
