theories/MetaTheory/Conversion/TermConversion.v
@@ -11,58 +11,76 @@ From Metaprog.MetaTheory Require Export Reduction.Confluence.
 (** * Conversion relation on terms. *)
 (***********************************************************************)
 
-Reserved Notation "Γ ⊢ t ≡ u"
+Reserved Notation "Σ ⊢ t ≡{ f } u"
   (at level 50, no associativity, t at next level, u at next level).
 
 (** Conversion relation on terms, defined as the smallest equivalence
     relation containing [red1]. *)
-Inductive conv {s} Σ : term s -> term s -> Prop :=
-| conv_of_red1 t1 t2 : Σ ⊢ t1 ~> t2 -> Σ ⊢ t1 ≡ t2
-| conv_refl t : Σ ⊢ t ≡ t
-| conv_sym t1 t2 : Σ ⊢ t1 ≡ t2 -> Σ ⊢ t2 ≡ t1
-| conv_trans t1 t2 t3 : Σ ⊢ t1 ≡ t2 -> Σ ⊢ t2 ≡ t3 -> Σ ⊢ t1 ≡ t3
+Inductive conv (flags : red_flags) (Σ : evar_map) {s} : term s -> term s -> Prop :=
+| conv_of_red1 t1 t2 : Σ ⊢ t1 ~>{flags} t2 -> Σ ⊢ t1 ≡{flags} t2
+| conv_refl t : Σ ⊢ t ≡{flags} t
+| conv_sym t1 t2 : Σ ⊢ t1 ≡{flags} t2 -> Σ ⊢ t2 ≡{flags} t1
+| conv_trans t1 t2 t3 : Σ ⊢ t1 ≡{flags} t2 -> Σ ⊢ t2 ≡{flags} t3 -> Σ ⊢ t1 ≡{flags} t3
 
-where "Σ ⊢ t ≡ u" := (conv Σ t u).
+where "Σ ⊢ t ≡{ f } u" := (conv f Σ t u).
 
 Derive Signature for conv.
 
-#[export] Instance conv_Reflexive s Σ : Reflexive (@conv s Σ).
+Notation "Σ ⊢ t ≡ u" := (conv red_flags_all Σ t u)
+  (at level 50, no associativity, t at next level, u at next level).
+
+(***********************************************************************)
+(** * Typeclass instances for setoid rewriting. *)
+(***********************************************************************)
+
+#[export] Instance conv_Reflexive flags Σ s : Reflexive (@conv flags Σ s).
 Proof. intros t. apply conv_refl. Qed.
 
-#[export] Instance conv_Symmetric s Σ : Symmetric (@conv s Σ).
+#[export] Instance conv_Symmetric flags Σ s : Symmetric (@conv flags Σ s).
 Proof. intros t1 t2. apply conv_sym. Qed.
 
-#[export] Instance conv_Transitive s Σ : Transitive (@conv s Σ).
+#[export] Instance conv_Transitive flags Σ s : Transitive (@conv flags Σ s).
 Proof. intros t. apply conv_trans. Qed.
 
-Lemma conv_of_red {s} Σ (t u : term s) :
-  Σ ⊢ t ~~> u -> Σ ⊢ t ≡ u.
+Lemma conv_of_red flags Σ {s} (t u : term s) :
+  Σ ⊢ t ~~>{flags} u -> Σ ⊢ t ≡{flags} u.
 Proof.
 intros H. induction H.
 - reflexivity.
 - rewrite IHred. now apply conv_of_red1.
 Qed.
 
-#[export] Instance subrelation_red1_conv s Σ :
-  subrelation (@red1 s Σ) (@conv s Σ).
+#[export] Instance subrelation_red1_conv flags Σ s :
+  subrelation (@red1 flags Σ s) (@conv flags Σ s).
 Proof. intros t u H. now apply conv_of_red1. Qed.
 
-#[export] Instance subrelation_red1_conv_flip s Σ :
-  subrelation (Basics.flip (@red1 s Σ)) (@conv s Σ).
+#[export] Instance subrelation_red1_conv_flip flags Σ s :
+  subrelation (Basics.flip (@red1 flags Σ s)) (@conv flags Σ s).
 Proof.
 intros t u H. unfold Basics.flip in H. symmetry.
 now apply conv_of_red1.
 Qed.
 
-#[export] Instance subrelation_red_conv s Σ :
-  subrelation (@red s Σ) (@conv s Σ).
+#[export] Instance subrelation_red_conv flags Σ s :
+  subrelation (@red flags Σ s) (@conv flags Σ s).
 Proof. intros t u H. now apply conv_of_red. Qed.
 
-#[export] Instance subrelation_red_conv_flip s Σ :
-  subrelation (Basics.flip (@red s Σ)) (@conv s Σ).
+#[export] Instance subrelation_red_conv_flip flags Σ s :
+  subrelation (Basics.flip (@red flags Σ s)) (@conv flags Σ s).
 Proof.
 intros t u H. unfold Basics.flip in H. symmetry.
 now apply conv_of_red.
+Qed.
+
+Lemma conv_extend_flags {flags1 flags2 Σ s} :
+  red_flags_incl flags1 flags2 ->
+  subrelation (@conv flags1 Σ s) (@conv flags2 Σ s).
+Proof.
+intros Hf t u H. induction H.
+- apply (red1_extend_flags Hf) in H. now constructor.
+- reflexivity.
+- now symmetry.
+- etransitivity ; eauto.
 Qed.
 
 (***********************************************************************)
@@ -71,16 +89,16 @@ Qed.
 
 (** The Church-Rosser lemma is a direct consequence of the confluence lemma.
     Using Church-Rosser, one can lift many lemmas from [red] to [conv]. *)
-Lemma church_rosser {s} Σ (t1 t2 : term s) :
-  Σ ⊢ t1 ≡ t2 ->
-  exists u, Σ ⊢ t1 ~~> u /\ Σ ⊢ t2 ~~> u.
+Lemma church_rosser {flags Σ s} (t1 t2 : term s) :
+  Σ ⊢ t1 ≡{flags} t2 ->
+  exists u, Σ ⊢ t1 ~~>{flags} u /\ Σ ⊢ t2 ~~>{flags} u.
 Proof.
 intros H. depind H.
 - exists t2. split ; [now apply red_of_red1 | reflexivity].
 - exists t. now split.
 - destruct IHconv as (u & H1 & H2). exists u. now split.
 - destruct IHconv1 as (u1 & H1 & H2). destruct IHconv2 as (u2 & H3 & H4).
-  destruct (red_confluence Σ t2 u1 u2 H2 H3) as (u & H5 & H6).
+  destruct (red_confluence t2 u1 u2 H2 H3) as (u & H5 & H6).
   exists u. split ; etransitivity ; eassumption.
 Qed.
 
@@ -89,14 +107,15 @@ Qed.
 (***********************************************************************)
 
 Section CongruenceLemmas.
-  Context {s : scope} (Σ : evar_map).
+  Context {flags : red_flags} {Σ : evar_map} {s : scope}.
 
   Lemma conv_beta x (ty : term s) body arg args :
-    Σ ⊢ TApp (TLam x ty body) (arg :: args) ≡ TApp (body[x := arg]) args.
-  Proof. now rewrite red_beta. Qed.
+    flags.(beta) = true ->
+    Σ ⊢ TApp (TLam x ty body) (arg :: args) ≡{flags} TApp (body[x := arg]) args.
+  Proof. intros H. now rewrite red_beta. Qed.
 
   #[export] Instance conv_lam_congr x :
-    Proper (conv Σ ==> conv Σ ==> conv Σ) (@TLam s x).
+    Proper (conv flags Σ ==> conv flags Σ ==> conv flags Σ) (@TLam s x).
   Proof.
   intros ty ty' Hty body body' Hbody. transitivity (TLam x ty' body).
   - clear Hbody. induction Hty.
@@ -112,7 +131,7 @@ Section CongruenceLemmas.
   Qed.
 
   #[export] Instance conv_prod_congr x :
-    Proper (conv Σ ==> conv Σ ==> conv Σ) (@TProd s x).
+    Proper (conv flags Σ ==> conv flags Σ ==> conv flags Σ) (@TProd s x).
   Proof.
   intros a a' Ha b b' Hb. transitivity (TProd x a' b).
   - clear Hb. induction Ha.
@@ -128,8 +147,8 @@ Section CongruenceLemmas.
   Qed.
 
   Lemma conv_app_congr_aux (f : term s) l (args args' : list (term s)) :
-    All2 (conv Σ) args args' ->
-    Σ ⊢ TApp f (l ++ args) ≡ TApp f (l ++ args').
+    All2 (conv flags Σ) args args' ->
+    Σ ⊢ TApp f (l ++ args) ≡{flags} TApp f (l ++ args').
   Proof.
   intros H. revert f l. depind H ; intros f l.
   - reflexivity.
@@ -144,7 +163,7 @@ Section CongruenceLemmas.
   Qed.
 
   #[export] Instance conv_app_congr :
-    Proper (conv Σ ==> All2 (conv Σ) ==> conv Σ) (@TApp s).
+    Proper (conv flags Σ ==> All2 (conv flags Σ) ==> conv flags Σ) (@TApp s).
   Proof.
   intros f f' Hf args arg' Hargs. transitivity (TApp f' args).
   - clear Hargs. induction Hf.
@@ -162,12 +181,12 @@ End CongruenceLemmas.
 (***********************************************************************)
 
 Section InversionLemmas.
-  Context {s : scope} (Σ : evar_map).
+  Context {flags : red_flags} {Σ : evar_map} {s : scope}.
 
   (** Injectivity of [TLam]. *)
   Lemma conv_lam_inv x (ty ty' : term s) body body' :
-    Σ ⊢ TLam x ty body ≡ TLam x ty' body' ->
-    Σ ⊢ ty ≡ ty' /\ Σ ⊢ body ≡ body'.
+    Σ ⊢ TLam x ty body ≡{flags} TLam x ty' body' ->
+    Σ ⊢ ty ≡{flags} ty' /\ Σ ⊢ body ≡{flags} body'.
   Proof.
   intros H. apply church_rosser in H. destruct H as (t & H1 & H2).
   apply red_lam_inv in H1, H2.
@@ -184,8 +203,8 @@ Section InversionLemmas.
 
   (** Injectivity of [TProd]. *)
   Lemma conv_prod_inv x (a a' : term s) b b' :
-    Σ ⊢ TProd x a b ≡ TProd x a' b' ->
-    Σ ⊢ a ≡ a' /\ Σ ⊢ b ≡ b'.
+    Σ ⊢ TProd x a b ≡{flags} TProd x a' b' ->
+    Σ ⊢ a ≡{flags} a' /\ Σ ⊢ b ≡{flags} b'.
   Proof.
   intros H. apply church_rosser in H. destruct H as (t & H1 & H2).
   apply red_prod_inv in H1, H2.
