theories/MetaTheory/Reduction/Confluence.v
@@ -9,77 +9,80 @@ From Metaprog.MetaTheory Require Export Reduction.ContextReduction.
     of contexts [cred]. *)
 
 (***********************************************************************)
-(** * Parallel reduction. *)
+(** * Parallel reduction on terms. *)
 (***********************************************************************)
 
-#[local] Reserved Notation "Σ ⊢ t >> u"
+#[local] Reserved Notation "Σ ⊢ t >>{ f } u"
   (at level 50, no associativity, t at next level, u at next level).
 
 Unset Elimination Schemes.
 
 (** Parallel reduction relation. *)
-Inductive pred1 {s} (Σ : evar_map) : term s -> term s -> Prop :=
+Inductive pred1 (flags : red_flags) (Σ : evar_map) {s} : term s -> term s -> Prop :=
 
 (** Beta-reduction rule. *)
 | pred1_app_beta x ty body body' arg arg' args args' :
-    Σ ⊢ body >> body' ->
-    Σ ⊢ arg >> arg' ->
-    All2 (pred1 Σ) args args' ->
-    Σ ⊢ TApp (TLam x ty body) (arg :: args) >> TApp (body'[x := arg']) args'
+    flags.(beta) = true ->
+    Σ ⊢ body >>{flags} body' ->
+    Σ ⊢ arg >>{flags} arg' ->
+    All2 (pred1 flags Σ) args args' ->
+    Σ ⊢ TApp (TLam x ty body) (arg :: args) >>{flags} TApp (body'[x := arg']) args'
 
 (** Evar expansion rule. *)
 | pred1_evar_expand ev ty def :
+    flags.(evars) = true ->
     Σ ev = Some (mk_evar_entry ty (Some def)) ->
-    Σ ⊢ TEvar ev >> wk def
+    Σ ⊢ TEvar ev >>{flags} wk def
 
 (** Congruence rules. *)
 
 | pred1_type :
-    Σ ⊢ TType >> TType
+    Σ ⊢ TType >>{flags} TType
 
 | pred1_var i :
-    Σ ⊢ TVar i >> TVar i
+    Σ ⊢ TVar i >>{flags} TVar i
 
 | pred1_lam x ty ty' body body' :
-    Σ ⊢ ty >> ty' ->
-    Σ ⊢ body >> body' ->
-    Σ ⊢ TLam x ty body >> TLam x ty' body'
+    Σ ⊢ ty >>{flags} ty' ->
+    Σ ⊢ body >>{flags} body' ->
+    Σ ⊢ TLam x ty body >>{flags} TLam x ty' body'
 
 | pred1_prod x a a' b b' :
-    Σ ⊢ a >> a' ->
-    Σ ⊢ b >> b' ->
-    Σ ⊢ TProd x a b >> TProd x a' b'
+    Σ ⊢ a >>{flags} a' ->
+    Σ ⊢ b >>{flags} b' ->
+    Σ ⊢ TProd x a b >>{flags} TProd x a' b'
 
 | pred1_app f f' args args' :
-    Σ ⊢ f >> f' ->
-    All2 (pred1 Σ) args args' ->
-    Σ ⊢ TApp f args >> TApp f' args'
+    Σ ⊢ f >>{flags} f' ->
+    All2 (pred1 flags Σ) args args' ->
+    Σ ⊢ TApp f args >>{flags} TApp f' args'
 
 | pred1_evar ev :
-    Σ ⊢ TEvar ev >> TEvar ev
+    Σ ⊢ TEvar ev >>{flags} TEvar ev
 
-where "Σ ⊢ t >> u" := (pred1 Σ t u).
+where "Σ ⊢ t >>{ f } u" := (pred1 f Σ t u).
 
 Set Elimination Schemes.
 
 Derive Signature for pred1.
 
-#[export] Instance pred1_Reflexive s Σ :
-  Reflexive (@pred1 s Σ).
+#[export] Instance pred1_Reflexive flags Σ s :
+  Reflexive (@pred1 flags Σ s).
 Proof.
 intros t. induction t using term_ind' ; constructor ; try assumption.
 induction args ; constructor ; depelim H ; auto.
 Qed.
 
+(***********************************************************************)
+(** * Parallel reduction on substitutions. *)
+(***********************************************************************)
+
 (** Parallel reduction on substitutions is just pointwise parallel reduction. *)
-Definition spred1 {s s'} Σ (σ σ' : subst s s') : Prop :=
-  forall i, Σ ⊢ sapply σ i >> sapply σ' i.
+Definition spred1 flags Σ {s s'} (σ σ' : subst s s') : Prop :=
+  forall i, Σ ⊢ sapply σ i >>{flags} sapply σ' i.
 
-Notation "Σ ⊢ σ1 >>ₛ σ2" := (spred1 Σ σ1 σ2)
-  (at level 50, no associativity, σ1 at next level, σ2 at next level).
-
-#[export] Instance spred1_Reflexive s s' Σ :
-  Reflexive (@spred1 s s' Σ).
+#[export] Instance spred1_Reflexive flags Σ s s' :
+  Reflexive (@spred1 flags Σ s s').
 Proof. intros σ i. reflexivity. Qed.
 
 (***********************************************************************)
@@ -88,41 +91,43 @@ Proof. intros σ i. reflexivity. Qed.
 
 (** Induction principle for [pred1]. We can't use Rocq's default induction principle
     because [pred1] is nested over [All2]. *)
-Lemma pred1_ind (P : forall s, evar_map -> term s -> term s -> Prop)
-  (Hbeta : forall s Σ x ty body body' arg arg' args args',
-    Σ ⊢ body >> body' -> P (s ▷ x) Σ body body' ->
-    Σ ⊢ arg >> arg' -> P s Σ arg arg' ->
-    All2 (pred1 Σ) args args' -> All2 (P s Σ) args args' ->
-    P s Σ (TApp (TLam x ty body) (arg :: args)) (TApp (body'[x := arg']) args'))
-  (Hexpand : forall s Σ ev ty def,
+Lemma pred1_ind flags Σ (P : forall s, term s -> term s -> Prop)
+  (Hbeta : forall s x ty body body' arg arg' args args',
+    flags.(beta) = true ->
+    Σ ⊢ body >>{flags} body' -> P (s ▷ x) body body' ->
+    Σ ⊢ arg >>{flags} arg' -> P s arg arg' ->
+    All2 (pred1 flags Σ) args args' -> All2 (P s) args args' ->
+    P s (TApp (TLam x ty body) (arg :: args)) (TApp (body'[x := arg']) args'))
+  (Hexpand : forall s ev ty def,
+    flags.(evars) = true ->
     Σ ev = Some (mk_evar_entry ty (Some def)) ->
-    P s Σ (TEvar ev) (wk def))
-  (Htype : forall s Σ,
-    P s Σ TType TType)
-  (Hvar : forall s Σ i,
-    P s Σ (TVar i) (TVar i))
-  (Hlam : forall s Σ x ty ty' body body',
-    Σ ⊢ ty >> ty' -> P s Σ ty ty' ->
-    Σ ⊢ body >> body' -> P (s ▷ x) Σ body body' ->
-    P s Σ (TLam x ty body) (TLam x ty' body'))
-  (Hprod : forall s Σ x a a' b b',
-    Σ ⊢ a >> a' -> P s Σ a a' ->
-    Σ ⊢ b >> b' -> P (s ▷ x) Σ b b' ->
-    P s Σ (TProd x a b) (TProd x a' b'))
-  (Happ : forall s Σ f f' args args',
-    Σ ⊢ f >> f' -> P s Σ f f' ->
-    All2 (pred1 Σ) args args' -> All2 (P s Σ) args args' ->
-    P s Σ (TApp f args) (TApp f' args'))
-  (Hevar : forall s Σ ev,
-    P s Σ (TEvar ev) (TEvar ev)) :
-  forall s Σ t t', Σ ⊢ t >> t' -> P s Σ t t'.
+    P s (TEvar ev) (wk def))
+  (Htype : forall s,
+    P s TType TType)
+  (Hvar : forall s i,
+    P s (TVar i) (TVar i))
+  (Hlam : forall s x ty ty' body body',
+    Σ ⊢ ty >>{flags} ty' -> P s ty ty' ->
+    Σ ⊢ body >>{flags} body' -> P (s ▷ x) body body' ->
+    P s (TLam x ty body) (TLam x ty' body'))
+  (Hprod : forall s x a a' b b',
+    Σ ⊢ a >>{flags} a' -> P s a a' ->
+    Σ ⊢ b >>{flags} b' -> P (s ▷ x) b b' ->
+    P s (TProd x a b) (TProd x a' b'))
+  (Happ : forall s f f' args args',
+    Σ ⊢ f >>{flags} f' -> P s f f' ->
+    All2 (pred1 flags Σ) args args' -> All2 (P s) args args' ->
+    P s (TApp f args) (TApp f' args'))
+  (Hevar : forall s ev,
+    P s (TEvar ev) (TEvar ev)) :
+  forall s t t', Σ ⊢ t >>{flags} t' -> P s t t'.
 Proof.
-fix IH 5. intros s Σ t t' Hred. destruct Hred.
+fix IH 4. intros s t t' Hred. destruct Hred.
 - apply Hbeta ; try assumption ; try now apply IH.
-  revert args args' H. fix IHargs 3. intros args args' H. destruct H.
+  revert args args' H0. fix IHargs 3. intros args args' H0. destruct H0.
   + constructor.
   + constructor ; auto.
-- apply Hexpand with ty. assumption.
+- apply Hexpand with ty ; assumption.
 - apply Htype.
 - apply Hvar.
 - apply Hlam ; auto.
@@ -137,329 +142,357 @@ Qed.
 (** * Relating parallel reduction and standard reduction. *)
 (***********************************************************************)
 
-(** [pred1] admits the beta rule. *)
-Lemma pred1_beta {s} Σ x (ty : term s) body arg args :
-  Σ ⊢ TApp (TLam x ty body) (arg :: args) >> TApp (body[x := arg]) args.
-Proof. now apply pred1_app_beta. Qed.
+Section RelatingPredRed.
+  Context {flags : red_flags} {Σ : evar_map}.
 
-(** One-step reduction is included in parallel reduction. *)
-Lemma pred1_of_red1 {s} Σ (t u : term s) :
-  Σ ⊢ t ~> u -> Σ ⊢ t >> u.
-Proof.
-intros H. induction H.
-- apply pred1_beta.
-- eapply pred1_evar_expand ; eassumption.
-- now apply pred1_lam.
-- now apply pred1_lam.
-- now apply pred1_prod.
-- now apply pred1_prod.
-- now apply pred1_app.
-- apply pred1_app ; [reflexivity|]. apply All2_of_OnOne2 ; [typeclasses eauto|].
-  revert H. apply OnOne2_consequence. firstorder.
-Qed.
+  (** [pred1] admits the beta rule. *)
+  Lemma pred1_beta {s} x (ty : term s) body arg args :
+    flags.(beta) = true ->
+    Σ ⊢ TApp (TLam x ty body) (arg :: args) >>{flags} TApp (body[x := arg]) args.
+  Proof. intros H. now apply pred1_app_beta. Qed.
 
-(** Parallel reduction is included in standard reduction. *)
-Lemma red_of_pred1 {s} Σ (t u : term s) :
-  Σ ⊢ t >> u -> Σ ⊢ t ~~> u.
-Proof.
-intros H. induction H.
-- rewrite <-red_beta. apply red_app_congr.
-  + now apply red_lam_congr.
-  + now constructor.
-- eapply red_evar_expand ; eassumption.
-- reflexivity.
-- reflexivity.
-- now apply red_lam_congr.
-- now apply red_prod_congr.
-- now apply red_app_congr.
-- reflexivity.
-Qed.
+  (** One-step reduction is included in parallel reduction. *)
+  Lemma pred1_of_red1 {s} (t u : term s) :
+    Σ ⊢ t ~>{flags} u -> Σ ⊢ t >>{flags} u.
+  Proof.
+  intros H. induction H.
+  - now apply pred1_beta.
+  - eapply pred1_evar_expand ; eassumption.
+  - now apply pred1_lam.
+  - now apply pred1_lam.
+  - now apply pred1_prod.
+  - now apply pred1_prod.
+  - now apply pred1_app.
+  - apply pred1_app ; [reflexivity|]. apply All2_of_OnOne2 ; [typeclasses eauto|].
+    revert H. apply OnOne2_consequence. firstorder.
+  Qed.
 
-(** The reflexive closure of [pred1] is equal to [red]. *)
-Lemma red_is_pred {s} Σ (t u : term s) :
-  Σ ⊢ t ~~> u <-> refl_trans_clos (pred1 Σ) t u.
-Proof.
-split ; intros H ; induction H.
-- reflexivity.
-- apply refl_trans_step with t2 ; auto. now apply pred1_of_red1.
-- reflexivity.
-- rewrite IHrefl_trans_clos. now apply red_of_pred1.
-Qed.
+  (** Parallel reduction is included in standard reduction. *)
+  Lemma red_of_pred1 {s} (t u : term s) :
+    Σ ⊢ t >>{flags} u -> Σ ⊢ t ~~>{flags} u.
+  Proof.
+  intros H. induction H.
+  - rewrite <-red_beta. apply red_app_congr.
+    + now apply red_lam_congr.
+    + now constructor.
+    + assumption.
+  - eapply red_evar_expand ; eassumption.
+  - reflexivity.
+  - reflexivity.
+  - now apply red_lam_congr.
+  - now apply red_prod_congr.
+  - now apply red_app_congr.
+  - reflexivity.
+  Qed.
+
+  (** The reflexive closure of [pred1] is equal to [red]. *)
+  Lemma red_is_pred {s} (t u : term s) :
+    Σ ⊢ t ~~>{flags} u <-> refl_trans_clos (pred1 flags Σ) t u.
+  Proof.
+  split ; intros H ; induction H.
+  - reflexivity.
+  - apply refl_trans_step with t2 ; auto. now apply pred1_of_red1.
+  - reflexivity.
+  - rewrite IHrefl_trans_clos. now apply red_of_pred1.
+  Qed.
+
+End RelatingPredRed.
 
 (***********************************************************************)
 (** * Compatibility with renaming and substitution. *)
 (***********************************************************************)
 
-Lemma pred1_app_beta_alt {s} Σ x (ty : term s) body body' arg arg' args args' t :
-  Σ ⊢ body >> body' ->
-  Σ ⊢ arg >> arg' ->
-  All2 (pred1 Σ) args args' ->
-  t = TApp (body' [x := arg']) args' ->
-  Σ ⊢ TApp (TLam x ty body) (arg :: args) >> t.
-Proof. intros H1 H2 H3 ->. now apply pred1_app_beta. Qed.
+Section Substitutivity.
+  Context {flags : red_flags} {Σ : evar_map}.
 
-(** Renaming lemma for [pred1]. *)
-#[export] Instance pred1_rename {s s'} Σ (ρ : ren s s') :
-  Proper (pred1 Σ ==> pred1 Σ) (rename ρ).
-Proof.
-intros t t' H. induction H in s', ρ |- * ; simpl_subst.
-- eapply pred1_app_beta_alt
-    with (body' := rename (rup x ρ) body')
-         (arg' := rename ρ arg')
-         (args' := map (rename ρ) args').
-  + auto.
-  + auto.
-  + change (All2 (pred1 Σ) (map (rename ρ) args) (map (rename ρ) args')).
-    rewrite All2_map. revert H2. apply All2_consequence. firstorder.
-  + now simpl_subst.
-- econstructor ; eassumption.
-- reflexivity.
-- reflexivity.
-- now apply pred1_lam.
-- now apply pred1_prod.
-- apply pred1_app.
-  + apply IHpred1.
-  + revert H1. rewrite All2_map. apply All2_consequence. firstorder.
-- reflexivity.
-Qed.
+  Lemma pred1_app_beta_alt {s} x (ty : term s) body body' arg arg' args args' t :
+    flags.(beta) = true ->
+    Σ ⊢ body >>{flags} body' ->
+    Σ ⊢ arg >>{flags} arg' ->
+    All2 (pred1 flags Σ) args args' ->
+    t = TApp (body' [x := arg']) args' ->
+    Σ ⊢ TApp (TLam x ty body) (arg :: args) >>{flags} t.
+  Proof. intros Hf H1 H2 H3 ->. now apply pred1_app_beta. Qed.
 
-#[export] Instance pred1_scons {x s s'} Σ :
-  Proper (pred1 Σ ==> spred1 Σ ==> spred1 Σ) (@scons s s' x).
-Proof. intros t t' Ht σ σ' Hσ i. depelim i ; simpl_subst ; auto. Qed.
+  (** Renaming lemma for [pred1]. *)
+  #[export] Instance pred1_rename {s s'} (ρ : ren s s') :
+    Proper (pred1 flags Σ ==> pred1 flags Σ) (rename ρ).
+  Proof.
+  intros t t' H. induction H in s', ρ |- * ; simpl_subst.
+  - eapply pred1_app_beta_alt
+      with (body' := rename (rup x ρ) body')
+           (arg' := rename ρ arg')
+           (args' := map (rename ρ) args') ;
+    auto.
+    + change (All2 (pred1 flags Σ) (map (rename ρ) args) (map (rename ρ) args')).
+      rewrite All2_map. revert H3. apply All2_consequence. firstorder.
+    + now simpl_subst.
+  - econstructor ; eassumption.
+  - reflexivity.
+  - reflexivity.
+  - now apply pred1_lam.
+  - now apply pred1_prod.
+  - apply pred1_app.
+    + apply IHpred1.
+    + revert H1. rewrite All2_map. apply All2_consequence. firstorder.
+  - reflexivity.
+  Qed.
 
-#[export] Instance pred1_sup {x s s'} Σ :
-  Proper (spred1 Σ ==> spred1 Σ) (@sup s s' x).
-Proof.
-intros σ σ' H i. depelim i ; simpl_subst.
-- reflexivity.
-- apply pred1_rename. apply H.
-Qed.
+  #[export] Instance pred1_scons {x s s'} :
+    Proper (pred1 flags Σ ==> spred1 flags Σ ==> spred1 flags Σ) (@scons s s' x).
+  Proof. intros t t' Ht σ σ' Hσ i. depelim i ; simpl_subst ; auto. Qed.
 
-(** Substitution lemma for [pred1]. *)
-#[export] Instance pred1_substitute {s s'} Σ :
-  Proper (spred1 Σ ==> pred1 Σ ==> pred1 Σ) (@substitute s s').
-Proof.
-intros σ σ' Hσ t t' Ht. induction Ht in s', σ, σ', Hσ |- * ; simpl_subst.
-- apply pred1_app_beta_alt
-    with (body' := substitute (sup x σ') body')
-         (arg' := substitute σ' arg')
-         (args' := map (substitute σ') args').
-  + apply IHHt1. now apply pred1_sup.
-  + now apply IHHt2.
-  + change (All2 (pred1 Σ) (map (substitute σ) args) (map (substitute σ') args')).
-    rewrite All2_map. revert H0. apply All2_consequence. firstorder.
-  + now simpl_subst.
-- econstructor ; eauto.
-- reflexivity.
-- apply Hσ.
-- apply pred1_lam ; auto. apply IHHt2. now apply pred1_sup.
-- apply pred1_prod ; auto. apply IHHt2. now apply pred1_sup.
-- apply pred1_app ; auto. rewrite All2_map. revert H0.
-  apply All2_consequence. firstorder.
-- reflexivity.
-Qed.
+  #[export] Instance pred1_sup {x s s'} :
+    Proper (spred1 flags Σ ==> spred1 flags Σ) (@sup s s' x).
+  Proof.
+  intros σ σ' H i. depelim i ; simpl_subst.
+  - reflexivity.
+  - apply pred1_rename. apply H.
+  Qed.
+
+  (** Substitution lemma for [pred1]. *)
+  #[export] Instance pred1_substitute {s s'} :
+    Proper (spred1 flags Σ ==> pred1 flags Σ ==> pred1 flags Σ) (@substitute s s').
+  Proof.
+  intros σ σ' Hσ t t' Ht. induction Ht in s', σ, σ', Hσ |- * ; simpl_subst.
+  - apply pred1_app_beta_alt
+      with (body' := substitute (sup x σ') body')
+           (arg' := substitute σ' arg')
+           (args' := map (substitute σ') args').
+    + assumption.
+    + apply IHHt1. now apply pred1_sup.
+    + now apply IHHt2.
+    + change (All2 (pred1 flags Σ) (map (substitute σ) args) (map (substitute σ') args')).
+      rewrite All2_map. revert H1. apply All2_consequence. firstorder.
+    + now simpl_subst.
+  - econstructor ; eauto.
+  - reflexivity.
+  - apply Hσ.
+  - apply pred1_lam ; auto. apply IHHt2. now apply pred1_sup.
+  - apply pred1_prod ; auto. apply IHHt2. now apply pred1_sup.
+  - apply pred1_app ; auto. rewrite All2_map. revert H0.
+    apply All2_consequence. firstorder.
+  - reflexivity.
+  Qed.
+
+End Substitutivity.
 
 (***********************************************************************)
 (** * Joinability for parallel reduction. *)
 (***********************************************************************)
 
 (** Two terms are joinable if they have a common reduct for [pred1]. *)
-Definition joinable {s} Σ (t1 t2 : term s) : Prop :=
-  exists u, Σ ⊢ t1 >> u /\ Σ ⊢ t2 >> u.
-
-#[export] Instance joinable_Reflexive s Σ :
-  Reflexive (@joinable s Σ).
-Proof. intros t. exists t. now split. Qed.
-
-#[export] Instance joinable_Symmetric s Σ :
-  Symmetric (@joinable s Σ).
-Proof. intros t1 t2. unfold joinable. firstorder. Qed.
+Definition joinable flags Σ {s} (t1 t2 : term s) : Prop :=
+  exists u, Σ ⊢ t1 >>{flags} u /\ Σ ⊢ t2 >>{flags} u.
 
 (** Two substitutions are joinable if they are pointwise joinable. *)
-Definition joinable_subst {s s'} Σ (σ1 σ2 : subst s s') : Prop :=
-  exists σ, Σ ⊢ σ1 >>ₛ σ /\ Σ ⊢ σ2 >>ₛ σ.
+Definition joinable_subst flags Σ {s s'} (σ1 σ2 : subst s s') : Prop :=
+  exists σ, spred1 flags Σ σ1 σ /\ spred1 flags Σ σ2 σ.
 
-#[export] Instance joinable_subst_Reflexive s s' Σ :
-  Reflexive (@joinable_subst s s' Σ).
-Proof. intros σ. exists σ. split ; reflexivity. Qed.
+Section JoinabilityLemmas.
+  Context {flags : red_flags} {Σ : evar_map}.
 
-#[export] Instance joinable_subst_Symmetric s s' Σ :
-  Symmetric (@joinable_subst s s' Σ).
-Proof. intros σ1 σ2 (σ & H1 & H2). exists σ. firstorder. Qed.
+  #[export] Instance joinable_Reflexive s :
+    Reflexive (@joinable flags Σ s).
+  Proof. intros t. exists t. now split. Qed.
 
-Lemma joinable_scons {x s s'} Σ t1 t2 (σ1 σ2 : subst s s') :
-  joinable Σ t1 t2 ->
-  joinable_subst Σ σ1 σ2 ->
-  joinable_subst Σ (scons x t1 σ1) (scons x t2 σ2).
-Proof.
-intros (t & Ht1 & Ht2) (σ & Hσ1 & Hσ2). exists (scons x t σ).
-split ; now apply pred1_scons.
-Qed.
+  #[export] Instance joinable_Symmetric s :
+    Symmetric (@joinable flags Σ s).
+  Proof. intros t1 t2. unfold joinable. firstorder. Qed.
 
-Lemma joinable_substitute {s s'} Σ (t1 t2 : term s) (σ1 σ2 : subst s s') :
-  joinable Σ t1 t2 ->
-  joinable_subst Σ σ1 σ2 ->
-  joinable Σ (substitute σ1 t1) (substitute σ2 t2).
-Proof.
-intros (t & Ht1 & Ht2) (σ & Hσ1 & Hσ2). exists (substitute σ t).
-split ; now apply pred1_substitute.
-Qed.
+  #[export] Instance joinable_subst_Reflexive s s' :
+    Reflexive (@joinable_subst flags Σ s s').
+  Proof. intros σ. exists σ. split ; reflexivity. Qed.
 
-Lemma joinable_lam {s x} Σ (ty1 ty2 : term s) body1 body2 :
-  joinable Σ ty1 ty2 ->
-  joinable Σ body1 body2 ->
-  joinable Σ (TLam x ty1 body1) (TLam x ty2 body2).
-Proof.
-intros (ty & Hty1 & Hty2) (body & Hbody1 & Hbody2).
-exists (TLam x ty body). split ; apply pred1_lam ; assumption.
-Qed.
+  #[export] Instance joinable_subst_Symmetric s s' :
+    Symmetric (@joinable_subst flags Σ s s').
+  Proof. intros σ1 σ2 (σ & H1 & H2). exists σ. firstorder. Qed.
 
-Lemma joinable_prod {s x} Σ (a1 a2 : term s) b1 b2 :
-  joinable Σ a1 a2 ->
-  joinable Σ b1 b2 ->
-  joinable Σ (TProd x a1 b1) (TProd x a2 b2).
-Proof.
-intros (a & Ha1 & Ha2) (b & Hb1 & Hb2).
-exists (TProd x a b). split ; apply pred1_prod ; assumption.
-Qed.
+  Lemma joinable_scons {x s s'} t1 t2 (σ1 σ2 : subst s s') :
+    joinable flags Σ t1 t2 ->
+    joinable_subst flags Σ σ1 σ2 ->
+    joinable_subst flags Σ (scons x t1 σ1) (scons x t2 σ2).
+  Proof.
+  intros (t & Ht1 & Ht2) (σ & Hσ1 & Hσ2). exists (scons x t σ).
+  split ; now apply pred1_scons.
+  Qed.
 
-Lemma joinable_list {s} Σ (args1 args2 : list (term s)) :
-  All2 (joinable Σ) args1 args2 ->
-  exists args, All2 (pred1 Σ) args1 args /\ All2 (pred1 Σ) args2 args.
-Proof.
-intros H. induction H.
-- exists []. split ; constructor.
-- destruct H as (z & Hx & Hy). destruct IHAll2 as (args & Hargs1 & Hargs2).
-  exists (z :: args). split ; constructor ; assumption.
-Qed.
+  Lemma joinable_substitute {s s'} (t1 t2 : term s) (σ1 σ2 : subst s s') :
+    joinable flags Σ t1 t2 ->
+    joinable_subst flags Σ σ1 σ2 ->
+    joinable flags Σ (substitute σ1 t1) (substitute σ2 t2).
+  Proof.
+  intros (t & Ht1 & Ht2) (σ & Hσ1 & Hσ2). exists (substitute σ t).
+  split ; now apply pred1_substitute.
+  Qed.
 
-Lemma joinable_app {s} Σ (f1 f2 : term s) args1 args2 :
-  joinable Σ f1 f2 ->
-  All2 (joinable Σ) args1 args2 ->
-  joinable Σ (TApp f1 args1) (TApp f2 args2).
-Proof.
-intros (f & Hf1 & Hf2) Hargs. apply joinable_list in Hargs.
-destruct Hargs as (args & Hargs1 & Hargs2).
-exists (TApp f args). split ; apply pred1_app ; assumption.
-Qed.
+  Lemma joinable_lam {s x} (ty1 ty2 : term s) body1 body2 :
+    joinable flags Σ ty1 ty2 ->
+    joinable flags Σ body1 body2 ->
+    joinable flags Σ (TLam x ty1 body1) (TLam x ty2 body2).
+  Proof.
+  intros (ty & Hty1 & Hty2) (body & Hbody1 & Hbody2).
+  exists (TLam x ty body). split ; apply pred1_lam ; assumption.
+  Qed.
 
-Lemma joinable_beta {s x} Σ ty2 body1 body2 (arg1 arg2 : term s) args1 args2 :
-  joinable Σ body1 body2 ->
-  joinable Σ arg1 arg2 ->
-  All2 (joinable Σ) args1 args2 ->
-  joinable Σ (TApp (body1[x := arg1]) args1) (TApp (TLam x ty2 body2) (arg2 :: args2)).
-Proof.
-intros (body & Hbody1 & Hbody2) (arg & Harg1 & Harg2) Hargs.
-apply joinable_list in Hargs. destruct Hargs as (args & Hargs1 & Hargs2).
-exists (TApp (body[x := arg]) args). split.
-- apply pred1_app.
-  + repeat f_equiv ; assumption.
-  + assumption.
-- now eapply pred1_app_beta.
-Qed.
+  Lemma joinable_prod {s x} (a1 a2 : term s) b1 b2 :
+    joinable flags Σ a1 a2 ->
+    joinable flags Σ b1 b2 ->
+    joinable flags Σ (TProd x a1 b1) (TProd x a2 b2).
+  Proof.
+  intros (a & Ha1 & Ha2) (b & Hb1 & Hb2).
+  exists (TProd x a b). split ; apply pred1_prod ; assumption.
+  Qed.
+
+  Lemma joinable_list {s} (args1 args2 : list (term s)) :
+    All2 (joinable flags Σ) args1 args2 ->
+    exists args, All2 (pred1 flags Σ) args1 args /\ All2 (pred1 flags Σ) args2 args.
+  Proof.
+  intros H. induction H.
+  - exists []. split ; constructor.
+  - destruct H as (z & Hx & Hy). destruct IHAll2 as (args & Hargs1 & Hargs2).
+    exists (z :: args). split ; constructor ; assumption.
+  Qed.
+
+  Lemma joinable_app {s} (f1 f2 : term s) args1 args2 :
+    joinable flags Σ f1 f2 ->
+    All2 (joinable flags Σ) args1 args2 ->
+    joinable flags Σ (TApp f1 args1) (TApp f2 args2).
+  Proof.
+  intros (f & Hf1 & Hf2) Hargs. apply joinable_list in Hargs.
+  destruct Hargs as (args & Hargs1 & Hargs2).
+  exists (TApp f args). split ; apply pred1_app ; assumption.
+  Qed.
+
+  Lemma joinable_beta {s x} ty2 body1 body2 (arg1 arg2 : term s) args1 args2 :
+    flags.(beta) = true ->
+    joinable flags Σ body1 body2 ->
+    joinable flags Σ arg1 arg2 ->
+    All2 (joinable flags Σ) args1 args2 ->
+    joinable flags Σ (TApp (body1[x := arg1]) args1) (TApp (TLam x ty2 body2) (arg2 :: args2)).
+  Proof.
+  intros Hf (body & Hbody1 & Hbody2) (arg & Harg1 & Harg2) Hargs.
+  apply joinable_list in Hargs. destruct Hargs as (args & Hargs1 & Hargs2).
+  exists (TApp (body[x := arg]) args). split.
+  - apply pred1_app.
+    + repeat f_equiv ; assumption.
+    + assumption.
+  - eapply pred1_app_beta ; eauto.
+  Qed.
+
+End JoinabilityLemmas.
 
 (***********************************************************************)
 (** * Diamond property for parallel reduction. *)
 (***********************************************************************)
 
-(** Just a weird consequence lemma for [All2] needed to prove the diamond property. *)
-Lemma All2_weird_consequence {A} (P Q R : A -> A -> Prop) xs ys zs :
-  (forall x y z, P y x -> Q y z -> R x z) ->
-  All2 P ys xs -> All2 Q ys zs -> All2 R xs zs.
-Proof.
-intros H HP HQ. revert zs HQ. depind HP ; intros zs HQ ; depelim HQ ; constructor.
-- firstorder.
-- firstorder.
-Qed.
+Section DiamondPred1.
+  Context {flags : red_flags} {Σ : evar_map}.
 
-(** [pred1] has the diamond property. *)
-Lemma pred1_diamond {s} Σ (t u1 u2 : term s) :
-  Σ ⊢ t >> u1 -> Σ ⊢ t >> u2 -> joinable Σ u1 u2.
-Proof.
-intros H1 H2. depind H1 ; depelim H2 ; try reflexivity.
-- apply joinable_app ; [apply joinable_substitute ; [| apply joinable_scons] |].
-  + now apply IHpred1_1.
-  + now apply IHpred1_2.
-  + reflexivity.
-  + revert H0 H1. apply All2_weird_consequence. firstorder.
-- depelim H2. depelim H1. eapply joinable_beta.
-  + now apply IHpred1_1.
-  + now apply IHpred1_2.
-  + revert H0 H2. apply All2_weird_consequence. firstorder.
-- rewrite H in H0. depelim H0. reflexivity.
-- exists (wk def). split ; [reflexivity |]. econstructor ; eassumption.
-- apply joinable_lam ; auto.
-- apply joinable_prod ; auto.
-- depelim H1. depelim H. depelim H1.
-  specialize (IHpred1 (TLam x ty' body')). feed IHpred1. { now apply pred1_lam. }
-  destruct IHpred1 as (z & Hz1 & Hz2). depelim Hz1. depelim Hz2.
-  symmetry. eapply joinable_beta.
-  + eexists ; eauto.
-  + symmetry. auto.
-  + revert H3 H2. apply All2_weird_consequence. firstorder.
-- apply joinable_app ; auto. revert H0 H3. apply All2_weird_consequence. firstorder.
-- exists (wk def). split ; [|reflexivity]. econstructor ; eassumption.
-Qed.
+  (** Just a weird consequence lemma for [All2] needed to prove the diamond property. *)
+  Lemma All2_weird_consequence {A} (P Q R : A -> A -> Prop) xs ys zs :
+    (forall x y z, P y x -> Q y z -> R x z) ->
+    All2 P ys xs -> All2 Q ys zs -> All2 R xs zs.
+  Proof.
+  intros H HP HQ. revert zs HQ. depind HP ; intros zs HQ ; depelim HQ ; constructor.
+  - firstorder.
+  - firstorder.
+  Qed.
 
-(** [pred1] is confluent. This is a consequence of the diamond property. *)
-Lemma pred1_confluence {s} Σ :
-  diamond (refl_trans_clos (@pred1 s Σ)) (refl_trans_clos (@pred1 s Σ)).
-Proof. apply diamond_confluence. intros t u1 u2. apply pred1_diamond. Qed.
+  (** [pred1] has the diamond property. *)
+  Lemma pred1_diamond_aux {s} (t u1 u2 : term s) :
+    Σ ⊢ t >>{flags} u1 -> Σ ⊢ t >>{flags} u2 -> joinable flags Σ u1 u2.
+  Proof.
+  intros H1 H2. depind H1 ; depelim H2 ; try reflexivity.
+  - apply joinable_app ; [apply joinable_substitute ; [| apply joinable_scons] |].
+    + now apply IHpred1_1.
+    + now apply IHpred1_2.
+    + reflexivity.
+    + revert H1 H3. apply All2_weird_consequence. firstorder.
+  - depelim H3. depelim H2. eapply joinable_beta.
+    + assumption.
+    + now apply IHpred1_1.
+    + now apply IHpred1_2.
+    + revert H1 H4. apply All2_weird_consequence. firstorder.
+  - rewrite H0 in H2. depelim H2. reflexivity.
+  - exists (wk def). split ; [reflexivity |]. econstructor ; eassumption.
+  - apply joinable_lam ; auto.
+  - apply joinable_prod ; auto.
+  - depelim H1. depelim H. depelim H1.
+    specialize (IHpred1 (TLam x ty' body')). feed IHpred1. { now apply pred1_lam. }
+    destruct IHpred1 as (z & Hz1 & Hz2). depelim Hz1. depelim Hz2.
+    symmetry. eapply joinable_beta.
+    + eassumption.
+    + eexists ; eauto.
+    + symmetry. auto.
+    + revert H4 H2. apply All2_weird_consequence. firstorder.
+  - apply joinable_app ; auto. revert H0 H3. apply All2_weird_consequence. firstorder.
+  - exists (wk def). split ; [|reflexivity]. econstructor ; eassumption.
+  Qed.
+
+  Lemma pred1_diamond {s} : diamond (@pred1 flags Σ s) (@pred1 flags Σ s).
+  Proof. intros t1 t2 u H1 H2. eapply pred1_diamond_aux ; eauto. Qed.
+
+End DiamondPred1.
 
 (***********************************************************************)
 (** * Main result: confluence of [red], [sred], and [cred]. *)
 (***********************************************************************)
 
-(** Confluence for [red] is an immediate result of confluence for [pred1]. *)
-Lemma red_confluence {s} Σ (t u1 u2 : term s) :
-  Σ ⊢ t ~~> u1 ->
-  Σ ⊢ t ~~> u2 ->
-  exists v, Σ ⊢ u1 ~~> v /\ Σ ⊢ u2 ~~> v.
-Proof.
-intros H1 H2. rewrite red_is_pred in H1, H2.
-pose proof (H := pred1_confluence Σ t u1 u2 H1 H2).
-destruct H as (v & Hv1 & Hv2). exists v. rewrite !red_is_pred. now split.
-Qed.
+Section Confluence.
+  Context {flags : red_flags} {Σ : evar_map}.
 
-(** Confluence for [sred] follows from confluence for [red]. *)
-Lemma sred_confluence {s s'} Σ (σ τ1 τ2 : subst s s') :
-  sred Σ σ τ1 ->
-  sred Σ σ τ2 ->
-  exists σ', sred Σ τ1 σ' /\ sred Σ τ2 σ'.
-Proof.
-intros H1 H2. induction s in s', σ, τ1, τ2, H1, H2 |- *.
-- exists (sren wk_idx). split ; constructor ; intros i ; depelim i.
-- specialize (IHs s' (rscomp rshift σ) (rscomp rshift τ1) (rscomp rshift τ2)).
-  forward IHs. { now rewrite H1. }
-  forward IHs. { now rewrite H2. }
-  destruct IHs as (σ' & Hσ1 & Hσ2).
-  assert (exists t, Σ ⊢ sapply τ1 I0 ~~> t /\ Σ ⊢ sapply τ2 I0 ~~> t) as (t & Ht1 & Ht2).
-  {
-    apply red_confluence with (sapply σ I0).
-    - now rewrite H1.
-    - now rewrite H2.
-  }
-  exists (scons x t σ'). split ; constructor ; intros i ; depelim i ; simpl_subst.
-  + apply Ht1.
-  + apply Hσ1.
-  + apply Ht2.
-  + apply Hσ2.
-Qed.
+  (** Confluence for [red] is an immediate result of the diamond property for [pred1]. *)
+  Lemma red_confluence {s} (t u1 u2 : term s) :
+    Σ ⊢ t ~~>{flags} u1 ->
+    Σ ⊢ t ~~>{flags} u2 ->
+    exists v, Σ ⊢ u1 ~~>{flags} v /\ Σ ⊢ u2 ~~>{flags} v.
+  Proof.
+  intros H1 H2. setoid_rewrite red_is_pred. rewrite red_is_pred in H1, H2.
+  eapply diamond_confluence with (R := @pred1 flags Σ s) ; eauto using pred1_diamond.
+  Qed.
 
-(** Confluence for [cred] follows from confluence for [red]. *)
-Lemma cred_confluence {s} Σ (Γ Γ1 Γ2 : context ∅ s) :
-  cred Σ Γ Γ1 ->
-  cred Σ Γ Γ2 ->
-  exists Γ', cred Σ Γ1 Γ' /\ cred Σ Γ2 Γ'.
-Proof.
-intros H1 H2. induction s in Γ, Γ1, Γ2, H1, H2 |- *.
-- depelim Γ ; depelim Γ1 ; depelim Γ2. exists CNil. split ; constructor.
-- depelim H1. depelim H2.
-  destruct (IHs _ _ _ H1 H2) as (Γ1 & HΓ & HΓ').
-  assert (exists ty1, Σ ⊢ ty' ~~> ty1 /\ Σ ⊢ ty'0 ~~> ty1) as (ty1 & Hty1 & Hty2).
-  { now apply red_confluence with ty. }
-  exists (CCons Γ1 x ty1). split ; constructor ; auto.
-Qed.
+  (** Confluence for [sred] follows from confluence for [red]. *)
+  Lemma sred_confluence {s s'} (σ τ1 τ2 : subst s s') :
+    sred flags Σ σ τ1 ->
+    sred flags Σ σ τ2 ->
+    exists σ', sred flags Σ τ1 σ' /\ sred flags Σ τ2 σ'.
+  Proof.
+  intros H1 H2. induction s in s', σ, τ1, τ2, H1, H2 |- *.
+  - exists (sren wk_idx). split ; constructor ; intros i ; depelim i.
+  - specialize (IHs s' (rscomp rshift σ) (rscomp rshift τ1) (rscomp rshift τ2)).
+    forward IHs. { now rewrite H1. }
+    forward IHs. { now rewrite H2. }
+    destruct IHs as (σ' & Hσ1 & Hσ2).
+    assert (exists t, Σ ⊢ sapply τ1 I0 ~~>{flags} t /\ Σ ⊢ sapply τ2 I0 ~~>{flags} t) as (t & Ht1 & Ht2).
+    {
+      apply red_confluence with (sapply σ I0).
+      - now rewrite H1.
+      - now rewrite H2.
+    }
+    exists (scons x t σ'). split ; constructor ; intros i ; depelim i ; simpl_subst.
+    + apply Ht1.
+    + apply Hσ1.
+    + apply Ht2.
+    + apply Hσ2.
+  Qed.
+
+  (** Confluence for [cred] follows from confluence for [red]. *)
+  Lemma cred_confluence {s} (Γ Γ1 Γ2 : context ∅ s) :
+    cred flags Σ Γ Γ1 ->
+    cred flags Σ Γ Γ2 ->
+    exists Γ', cred flags Σ Γ1 Γ' /\ cred flags Σ Γ2 Γ'.
+  Proof.
+  intros H1 H2. induction s in Γ, Γ1, Γ2, H1, H2 |- *.
+  - depelim Γ ; depelim Γ1 ; depelim Γ2. exists CNil. split ; constructor.
+  - depelim H1. depelim H2.
+    destruct (IHs _ _ _ H1 H2) as (Γ1 & HΓ & HΓ').
+    assert (exists ty1, Σ ⊢ ty' ~~>{flags} ty1 /\ Σ ⊢ ty'0 ~~>{flags} ty1) as (ty1 & Hty1 & Hty2).
+    { now apply red_confluence with ty. }
+    exists (CCons Γ1 x ty1). split ; constructor ; auto.
+  Qed.
+
+End Confluence.
 
 
 
