theories/MetaTheory/Reduction/ContextReduction.v
@@ -13,57 +13,50 @@ From Metaprog Require Export Data.Context MetaTheory.Reduction.SubstReduction.
 (** * One-step reduction of contexts. *)
 (***********************************************************************)
 
-(** [cred1 Σ Γ Γ'] means that context [Γ] reduces to context [Γ'] in
+(** [cred1 flags Σ Γ Γ'] means that context [Γ] reduces to context [Γ'] in
     exactly one reduction step. *)
-Inductive cred1 (Σ : evar_map) : forall {s}, context ∅ s -> context ∅ s -> Prop :=
+Inductive cred1 (flags : red_flags) (Σ : evar_map) : forall {s}, context ∅ s -> context ∅ s -> Prop :=
 | cred1_head {s} Γ x (ty ty' : term s) :
-    Σ ⊢ ty ~> ty' ->
-    cred1 Σ (CCons Γ x ty) (CCons Γ x ty')
+    Σ ⊢ ty ~>{flags} ty' ->
+    cred1 flags Σ (CCons Γ x ty) (CCons Γ x ty')
 
 | cred1_tail {s} Γ Γ' x (ty : term s) :
-    cred1 Σ Γ Γ' ->
-    cred1 Σ (CCons Γ x ty) (CCons Γ' x ty).
+    cred1 flags Σ Γ Γ' ->
+    cred1 flags Σ (CCons Γ x ty) (CCons Γ' x ty).
 
 Derive Signature for cred1.
-
-Lemma lookup_context_cred1 {s Σ} (i : index s) Γ Γ' :
-  cred1 Σ Γ Γ' ->
-  Σ ⊢ lookup_context i Γ ~> lookup_context i Γ' \/
-  lookup_context i Γ = lookup_context i Γ'.
-Proof.
-intros Hred. induction Hred ; depelim i ; simp lookup_context ; simpl_subst.
-- left. now apply red1_rename.
-- now right.
-- now right.
-- destruct (IHHred i) as [H1 | H2].
-  + left. apply red1_rename. apply H1.
-  + right. now rewrite H2.
-Qed.
 
 (***********************************************************************)
 (** * Multi-step reduction of contexts. *)
 (***********************************************************************)
 
-(** [cred Σ Γ Γ'] means that context [Γ] reduces to context [Γ'] in
-    zero or more reduction step. *)
-Inductive cred (Σ : evar_map) : forall {s}, context ∅ s -> context ∅ s -> Prop :=
-| cred_nil : cred Σ CNil CNil
+(** [cred flags Σ Γ Γ'] means that context [Γ] reduces to context [Γ'] in
+    zero or more reduction step.
+
+    Note that we do not define [cred] as the reflexive-transitive closure
+    of [cred1]: this fact is instead expressed by the lemma [cred_ind_alt]. *)
+Inductive cred (flags : red_flags) (Σ : evar_map) : forall {s}, context ∅ s -> context ∅ s -> Prop :=
+| cred_nil : cred flags Σ CNil CNil
 
 | cred_cons {s} x (ty ty' : term s) Γ Γ' :
-    Σ ⊢ ty ~~> ty' ->
-    cred Σ Γ Γ' ->
-    cred Σ (CCons Γ x ty) (CCons Γ' x ty').
+    Σ ⊢ ty ~~>{flags} ty' ->
+    cred flags Σ Γ Γ' ->
+    cred flags Σ (CCons Γ x ty) (CCons Γ' x ty').
 
 Derive Signature for cred.
 
-#[export] Instance cred_Reflexive Σ s : Reflexive (@cred Σ s).
+(***********************************************************************)
+(** * Typeclass instances for setoid rewriting. *)
+(***********************************************************************)
+
+#[export] Instance cred_Reflexive flags Σ s : Reflexive (@cred flags Σ s).
 Proof.
 intros Γ. induction Γ ; constructor.
 - reflexivity.
 - assumption.
 Qed.
 
-#[export] Instance cred_Transitive Σ s : Transitive (@cred Σ s).
+#[export] Instance cred_Transitive flags Σ s : Transitive (@cred flags Σ s).
 Proof.
 intros Γ1 Γ2 Γ3 H1 H2. induction H1 ; depelim H2.
 - reflexivity.
@@ -72,7 +65,7 @@ intros Γ1 Γ2 Γ3 H1 H2. induction H1 ; depelim H2.
   + now apply IHcred.
 Qed.
 
-#[export] Instance cred_of_cred1 Σ s : subrelation (@cred1 Σ s) (@cred Σ s).
+#[export] Instance cred_of_cred1 flags Σ s : subrelation (@cred1 flags Σ s) (@cred flags Σ s).
 Proof.
 intros Γ Γ' HΓ. induction HΓ ; constructor.
 - now rewrite H.
@@ -81,54 +74,97 @@ intros Γ Γ' HΓ. induction HΓ ; constructor.
 - assumption.
 Qed.
 
-Lemma cred_is_clos_cred1_aux1 {s x} Σ (Γ Γ' : context ∅ s) ty :
-  refl_trans_clos (cred1 Σ) Γ Γ' ->
-  refl_trans_clos (cred1 Σ) (CCons Γ x ty) (CCons Γ' x ty).
+Lemma cred1_extend_flags {flags1 flags2 Σ s} :
+  red_flags_incl flags1 flags2 ->
+  subrelation (@cred1 flags1 Σ s) (@cred1 flags2 Σ s).
 Proof.
-intros H. induction H.
-- reflexivity.
-- rewrite IHrefl_trans_clos. apply refl_trans_clos_one. now constructor.
+intros Hf Γ Γ' HΓ. induction HΓ.
+- constructor. eapply red1_extend_flags ; eassumption.
+- constructor. assumption.
 Qed.
 
-Lemma cred_is_clos_cred1_aux2 {s x} Σ (Γ : context ∅ s) ty ty' :
-  Σ ⊢ ty ~> ty' ->
-  refl_trans_clos (cred1 Σ) (CCons Γ x ty) (CCons Γ x ty').
-Proof. intros H. apply refl_trans_clos_one. now constructor. Qed.
-
-Lemma cred_is_clos_cred1 {s} Σ (Γ Γ' : context ∅ s) :
-  cred Σ Γ Γ' <-> refl_trans_clos (cred1 Σ) Γ Γ'.
+Lemma cred_extend_flags {flags1 flags2 Σ s} :
+  red_flags_incl flags1 flags2 ->
+  subrelation (@cred flags1 Σ s) (@cred flags2 Σ s).
 Proof.
-split ; intros H.
-- induction H.
-  + reflexivity.
-  + induction H.
-    * now apply cred_is_clos_cred1_aux1.
-    * rewrite IHred. now apply cred_is_clos_cred1_aux2.
-- induction H.
-  + reflexivity.
-  + rewrite IHrefl_trans_clos, H0. reflexivity.
+intros Hf Γ Γ' HΓ. induction HΓ ; constructor.
+- eapply red_extend_flags ; eassumption.
+- assumption.
 Qed.
+
+(***********************************************************************)
+(** * Lemmas about context reduction. *)
+(***********************************************************************)
+
+Section Lemmas.
+  Context {flags : red_flags} {Σ : evar_map}.
+
+  Lemma lookup_context_cred1 {s} (i : index s) Γ Γ' :
+    cred1 flags Σ Γ Γ' ->
+    Σ ⊢ lookup_context i Γ ~>{flags} lookup_context i Γ' \/
+    lookup_context i Γ = lookup_context i Γ'.
+  Proof.
+  intros Hred. induction Hred ; depelim i ; simp lookup_context ; simpl_subst.
+  - left. now apply red1_rename.
+  - now right.
+  - now right.
+  - destruct (IHHred i) as [H1 | H2].
+    + left. apply red1_rename. apply H1.
+    + right. now rewrite H2.
+  Qed.
+
+  Lemma lookup_context_cred {s} (i : index s) Γ Γ' :
+    cred flags Σ Γ Γ' ->
+    Σ ⊢ lookup_context i Γ ~~>{flags} lookup_context i Γ'.
+  Proof.
+  intros H. induction H ; depelim i ; simp lookup_context ; simpl_subst.
+  - now rewrite H.
+  - now rewrite IHcred.
+  Qed.
+
+  Lemma cred_is_clos_cred1_aux1 {s x} (Γ Γ' : context ∅ s) ty :
+    refl_trans_clos (cred1 flags Σ) Γ Γ' ->
+    refl_trans_clos (cred1 flags Σ) (CCons Γ x ty) (CCons Γ' x ty).
+  Proof.
+  intros H. induction H.
+  - reflexivity.
+  - rewrite IHrefl_trans_clos. apply refl_trans_clos_one. now constructor.
+  Qed.
+
+  Lemma cred_is_clos_cred1_aux2 {s x} (Γ : context ∅ s) ty ty' :
+    Σ ⊢ ty ~>{flags} ty' ->
+    refl_trans_clos (cred1 flags Σ) (CCons Γ x ty) (CCons Γ x ty').
+  Proof. intros H. apply refl_trans_clos_one. now constructor. Qed.
+
+  (** [cred] is the reflexive-transitive closure of [cred1].
+      The lemma [cred_ind_alt] is usually more useful. *)
+  Lemma cred_is_clos_cred1 {s} (Γ Γ' : context ∅ s) :
+    cred flags Σ Γ Γ' <-> refl_trans_clos (cred1 flags Σ) Γ Γ'.
+  Proof.
+  split ; intros H.
+  - induction H.
+    + reflexivity.
+    + induction H.
+      * now apply cred_is_clos_cred1_aux1.
+      * rewrite IHred. now apply cred_is_clos_cred1_aux2.
+  - induction H.
+    + reflexivity.
+    + rewrite IHrefl_trans_clos, H0. reflexivity.
+  Qed.
+
+End Lemmas.
 
 (** Alternate induction principle for [cred] which expresses the fact that
     [cred] is the reflexive-transitive closure of [cred1]. *)
-Lemma cred_ind_alt (Σ : evar_map) (P : forall s, context ∅ s -> context ∅ s -> Prop)
+Lemma cred_ind_alt flags Σ (P : forall s, context ∅ s -> context ∅ s -> Prop)
   (Hrefl : forall s Γ, P s Γ Γ)
   (Hstep : forall s Γ1 Γ2 Γ3,
-    cred Σ Γ1 Γ2 -> P s Γ1 Γ2 ->
-    cred1 Σ Γ2 Γ3 ->
+    cred flags Σ Γ1 Γ2 -> P s Γ1 Γ2 ->
+    cred1 flags Σ Γ2 Γ3 ->
     P s Γ1 Γ3) :
-  forall s Γ1 Γ2, cred Σ Γ1 Γ2 -> P s Γ1 Γ2.
+  forall s Γ1 Γ2, cred flags Σ Γ1 Γ2 -> P s Γ1 Γ2.
 Proof.
 intros s Γ1 Γ2 H. rewrite cred_is_clos_cred1 in H. induction H.
 - apply Hrefl.
 - apply Hstep with y ; auto. now rewrite cred_is_clos_cred1.
-Qed.
-
-Lemma lookup_context_cred {s Σ} (i : index s) Γ Γ' :
-  cred Σ Γ Γ' ->
-  Σ ⊢ lookup_context i Γ ~~> lookup_context i Γ'.
-Proof.
-intros H. induction H ; depelim i ; simp lookup_context ; simpl_subst.
-- now rewrite H.
-- now rewrite IHcred.
 Qed.
