theories/MetaTheory/Reduction/SubstReduction.v
@@ -11,126 +11,140 @@ From Metaprog Require Export MetaTheory.Reduction.TermReduction.
 (***********************************************************************)
 
 (** Reduction on substitutions is just pointwise reduction.
+
     We wrap the definition in a record because otherwise rewriting with
-    [H : sred Σ σ σ'] will sometimes fail due to setoid rewrite wanting to rewrite
-    [sapply σ i] into [sapply σ' i].  *)
-Record sred {s s'} Σ (σ σ' : subst s s') := {
-  sred_prop : forall i, Σ ⊢ sapply σ i ~~> sapply σ' i
+    [H : sred flags Σ σ σ'] will sometimes fail due to setoid rewrite
+    wanting to rewrite [sapply σ i] into [sapply σ' i].  *)
+Record sred flags Σ {s s'} (σ σ' : subst s s') := {
+  sred_prop : forall i, Σ ⊢ sapply σ i ~~>{flags} sapply σ' i
 }.
 
-#[export] Instance sred_Reflexive s s' Σ : Reflexive (@sred s s' Σ).
+(***********************************************************************)
+(** * Typeclass instances for setoid rewriting. *)
+(***********************************************************************)
+
+#[export] Instance sred_Reflexive flags Σ s s' : Reflexive (@sred flags Σ s s').
 Proof. intros σ. constructor. reflexivity. Qed.
 
-#[export] Instance sred_Transitive s s' Σ : Transitive (@sred s s' Σ).
+#[export] Instance sred_Transitive flags Σ s s' : Transitive (@sred flags Σ s s').
 Proof.
 intros σ1 σ2 σ3 [H1] [H2]. constructor. intros i. etransitivity ; eauto.
 Qed.
 
-#[export] Instance red_sapply {s s'} Σ :
-  Proper (sred Σ ==> eq ==> red Σ) (@sapply s s').
+#[export] Instance red_sapply flags Σ s s' :
+  Proper (sred flags Σ ==> eq ==> red flags Σ) (@sapply s s').
 Proof. intros σ σ' [Hσ] i ? <-. apply Hσ. Qed.
 
-(***********************************************************************)
-(** * Compatibility of reduction with renaming. *)
-(***********************************************************************)
-
-(** Compatibility of renaming with [red1]. *)
-#[export] Instance red1_rename {Σ s s'} (ρ : ren s s') :
-  Proper (red1 Σ ==> red1 Σ) (rename ρ).
+Lemma sred_extend_flags {flags1 flags2 Σ s s'} :
+  red_flags_incl flags1 flags2 ->
+  subrelation (@sred flags1 Σ s s') (@sred flags2 Σ s s').
 Proof.
-intros t t' H. induction H in s', ρ |- * ; simpl_subst.
-- cbn. apply red1_beta_alt. f_equal. now simpl_subst.
-- eapply red1_evar_expand. eassumption.
-- now apply red1_lam_l.
-- now apply red1_lam_r.
-- now apply red1_prod_l.
-- now apply red1_prod_r.
-- now apply red1_app_l.
-- apply red1_app_r, OnOne2_map. revert H. apply OnOne2_consequence. firstorder.
-Qed.
-
-(** Compatibility of renaming with [red]. *)
-#[export] Instance red_rename {Σ s s'} (ρ : ren s s') :
-  Proper (red Σ ==> red Σ) (rename ρ).
-Proof.
-intros t t' H. induction H.
-- reflexivity.
-- now rewrite IHred, H0.
+intros Hf σ1 σ2 [Hσ]. constructor. intros i.
+eapply red_extend_flags ; eauto.
 Qed.
 
 (***********************************************************************)
-(** * Compatibility of reduction with substitution. *)
+(** * Compatibility of reduction with renaming and substitution. *)
 (***********************************************************************)
 
-#[export] Instance red_scons {Σ s s' x} :
-  Proper (red Σ ==> sred Σ ==> sred Σ) (@scons s s' x).
-Proof.
-intros t t' Ht σ σ' Hσ. constructor. intros i. depelim i ; simpl_subst.
-- assumption.
-- now rewrite Hσ.
-Qed.
+Section Substitutivity.
+  Context {flags : red_flags} {Σ : evar_map}.
 
-#[export] Instance red_srcomp {Σ s s' s''} :
-  Proper (sred Σ ==> eq ==> sred Σ) (@srcomp s s' s'').
-Proof.
-intros σ σ' Hσ ρ ρ' <-. constructor. intros i. simpl_subst.
-now rewrite Hσ.
-Qed.
+  (** Compatibility of renaming with [red1]. *)
+  #[export] Instance red1_rename {s s'} (ρ : ren s s') :
+    Proper (red1 flags Σ ==> red1 flags Σ) (rename ρ).
+  Proof.
+  intros t t' H. induction H in s', ρ |- * ; simpl_subst.
+  - cbn. apply red1_beta_alt ; auto. f_equal. now simpl_subst.
+  - eapply red1_evar_expand ; auto. eassumption.
+  - now apply red1_lam_l.
+  - now apply red1_lam_r.
+  - now apply red1_prod_l.
+  - now apply red1_prod_r.
+  - now apply red1_app_l.
+  - apply red1_app_r, OnOne2_map. revert H. apply OnOne2_consequence. firstorder.
+  Qed.
 
-#[export] Instance red_rscomp {Σ s s' s''} ρ :
-  Proper (sred Σ ==> sred Σ) (@rscomp s s' s'' ρ).
-Proof.
-intros σ σ' Hσ. constructor. intros i. simpl_subst.
-now rewrite Hσ.
-Qed.
+  (** Compatibility of renaming with [red]. *)
+  #[export] Instance red_rename {s s'} (ρ : ren s s') :
+    Proper (red flags Σ ==> red flags Σ) (rename ρ).
+  Proof.
+  intros t t' H. induction H.
+  - reflexivity.
+  - now rewrite IHred, H0.
+  Qed.
 
-#[export] Instance red_sup {Σ s s' x} :
-  Proper (sred Σ ==> sred Σ) (@sup s s' x).
-Proof. intros σ σ' Hσ. unfold sup. now rewrite Hσ. Qed.
+  #[export] Instance red_scons {s s' x} :
+    Proper (red flags Σ ==> sred flags Σ ==> sred flags Σ) (@scons s s' x).
+  Proof.
+  intros t t' Ht σ σ' Hσ. constructor. intros i. depelim i ; simpl_subst.
+  - assumption.
+  - now rewrite Hσ.
+  Qed.
 
-(** Compatibility of substitution with [red1]. Note that a single reduction in
-    the substitution can cause several reductions in the result, so here we fix
-    the substitution [σ]. *)
-#[export] Instance red1_substitute_l {Σ s s'} (σ : subst s s') :
-  Proper (red1 Σ ==> red1 Σ) (substitute σ).
-Proof.
-intros t t' H. induction H in s', σ |- * ; simpl_subst.
-- cbn. apply red1_beta_alt. f_equal. now simpl_subst.
-- eapply red1_evar_expand. eassumption.
-- now apply red1_lam_l.
-- now apply red1_lam_r.
-- now apply red1_prod_l.
-- now apply red1_prod_r.
-- now apply red1_app_l.
-- apply red1_app_r, OnOne2_map. revert H. apply OnOne2_consequence. firstorder.
-Qed.
+  #[export] Instance red_srcomp {s s' s''} :
+    Proper (sred flags Σ ==> eq ==> sred flags Σ) (@srcomp s s' s'').
+  Proof.
+  intros σ σ' Hσ ρ ρ' <-. constructor. intros i. simpl_subst.
+  now rewrite Hσ.
+  Qed.
 
-(** Substitution lemma for [red]. *)
-#[export] Instance red_substitute {Σ s s'} :
-  Proper (sred Σ ==> red Σ ==> red Σ) (@substitute s s').
-Proof.
-intros σ σ' Hσ t t' H. transitivity (substitute σ' t).
-- clear t' H. induction t in s', σ, σ', Hσ |- * using term_ind' ; simpl_subst.
-  + reflexivity.
-  + now rewrite Hσ.
-  + f_equiv.
-    * now apply IHt1.
-    * apply IHt2. now f_equiv.
-  + f_equiv.
-    * now apply IHt1.
-    * apply IHt2. now f_equiv.
-  + f_equiv.
-    * now apply IHt.
-    * clear t IHt. induction H ; cbn ; constructor ; auto.
-  + reflexivity.
-- induction H.
-  + reflexivity.
-  + now rewrite IHred, H0.
-Qed.
+  #[export] Instance red_rscomp {s s' s''} ρ :
+    Proper (sred flags Σ ==> sred flags Σ) (@rscomp s s' s'' ρ).
+  Proof.
+  intros σ σ' Hσ. constructor. intros i. simpl_subst.
+  now rewrite Hσ.
+  Qed.
 
-#[export] Instance red_scomp {Σ s s' s''} :
-  Proper (sred Σ ==> sred Σ ==> sred Σ) (@scomp s s' s'').
-Proof.
-intros σ σ' Hσ τ τ' Hτ. constructor. intros i. simpl_subst.
-now rewrite Hτ, Hσ.
-Qed.
+  #[export] Instance red_sup {s s' x} :
+    Proper (sred flags Σ ==> sred flags Σ) (@sup s s' x).
+  Proof. intros σ σ' Hσ. unfold sup. now rewrite Hσ. Qed.
+
+  (** Compatibility of substitution with [red1]. Note that a single reduction in
+      the substitution can cause several reductions in the result, so here we fix
+      the substitution [σ]. *)
+  #[export] Instance red1_substitute_l {s s'} (σ : subst s s') :
+    Proper (red1 flags Σ ==> red1 flags Σ) (substitute σ).
+  Proof.
+  intros t t' H. induction H in s', σ |- * ; simpl_subst.
+  - cbn. apply red1_beta_alt ; [assumption|]. f_equal. now simpl_subst.
+  - eapply red1_evar_expand ; [assumption|]. eassumption.
+  - now apply red1_lam_l.
+  - now apply red1_lam_r.
+  - now apply red1_prod_l.
+  - now apply red1_prod_r.
+  - now apply red1_app_l.
+  - apply red1_app_r, OnOne2_map. revert H. apply OnOne2_consequence. firstorder.
+  Qed.
+
+  (** Substitution lemma for [red]. *)
+  #[export] Instance red_substitute {s s'} :
+    Proper (sred flags Σ ==> red flags Σ ==> red flags Σ) (@substitute s s').
+  Proof.
+  intros σ σ' Hσ t t' H. transitivity (substitute σ' t).
+  - clear t' H. induction t in s', σ, σ', Hσ |- * using term_ind' ; simpl_subst.
+    + reflexivity.
+    + now rewrite Hσ.
+    + f_equiv.
+      * now apply IHt1.
+      * apply IHt2. now f_equiv.
+    + f_equiv.
+      * now apply IHt1.
+      * apply IHt2. now f_equiv.
+    + f_equiv.
+      * now apply IHt.
+      * clear t IHt. induction H ; cbn ; constructor ; auto.
+    + reflexivity.
+  - induction H.
+    + reflexivity.
+    + now rewrite IHred, H0.
+  Qed.
+
+  #[export] Instance red_scomp {s s' s''} :
+    Proper (sred flags Σ ==> sred flags Σ ==> sred flags Σ) (@scomp s s' s'').
+  Proof.
+  intros σ σ' Hσ τ τ' Hτ. constructor. intros i. simpl_subst.
+  now rewrite Hτ, Hσ.
+  Qed.
+
+End Substitutivity.
