theories/MetaTheory/Reduction/TermReduction.v
@@ -1,5 +1,5 @@
 From Metaprog Require Import Prelude.
-From Metaprog.MetaTheory Require Export Substitution EvarMap.
+From Metaprog.MetaTheory Require Export Substitution EvarMap RedFlags.
 
 (** This module defines:
     - The one-step strong reduction relation [red1] on terms.
@@ -13,46 +13,51 @@ From Metaprog.MetaTheory Require Export Substitution EvarMap.
 (** * One-step reduction relation [red1]. *)
 (***********************************************************************)
 
-Reserved Notation "Σ ⊢ t ~> u"
+Reserved Notation "Σ ⊢ t ~>{ f } u"
   (at level 50, no associativity, t at next level, u at next level).
 
 Unset Elimination Schemes.
 
 (** Strong one-step reduction relation. This relation is _not_ deterministic. *)
-Inductive red1 {s} Σ : term s -> term s -> Prop :=
+Inductive red1 (flags : red_flags) (Σ : evar_map) {s} : term s -> term s -> Prop :=
 
 (** Beta-reduction rule. *)
 | red1_beta x ty body arg args :
-    Σ ⊢ TApp (TLam x ty body) (arg :: args) ~> TApp (body[x := arg]) args
+    flags.(beta) = true ->
+    Σ ⊢ TApp (TLam x ty body) (arg :: args) ~>{flags} TApp (body[x := arg]) args
 
 (** Evar expansion. *)
 | red1_evar_expand ev ty def :
+    flags.(evars) = true ->
     Σ ev = Some (mk_evar_entry ty (Some def)) ->
-    Σ ⊢ TEvar ev ~> wk def
+    Σ ⊢ TEvar ev ~>{flags} wk def
 
 (** Congrence rules for [TLam]. *)
 | red1_lam_l x ty ty' body :
-    Σ ⊢ ty ~> ty' -> Σ ⊢ TLam x ty body ~> TLam x ty' body
+    Σ ⊢ ty ~>{flags} ty' -> Σ ⊢ TLam x ty body ~>{flags} TLam x ty' body
 | red1_lam_r x ty body body' :
-    Σ ⊢ body ~> body' -> Σ ⊢ TLam x ty body ~> TLam x ty body'
+    Σ ⊢ body ~>{flags} body' -> Σ ⊢ TLam x ty body ~>{flags} TLam x ty body'
 
 (** Congruence rules for [TProd]. *)
 | red1_prod_l x a a' b :
-    Σ ⊢ a ~> a' -> Σ ⊢ TProd x a b ~> TProd x a' b
+    Σ ⊢ a ~>{flags} a' -> Σ ⊢ TProd x a b ~>{flags} TProd x a' b
 | red1_prod_r x a b b' :
-    Σ ⊢ b ~> b' -> Σ ⊢ TProd x a b ~> TProd x a b'
+    Σ ⊢ b ~>{flags} b' -> Σ ⊢ TProd x a b ~>{flags} TProd x a b'
 
 (** Congruence rules for [TApp]. *)
 | red1_app_l f f' args :
-    Σ ⊢ f ~> f' -> Σ ⊢ TApp f args ~> TApp f' args
+    Σ ⊢ f ~>{flags} f' -> Σ ⊢ TApp f args ~>{flags} TApp f' args
 | red1_app_r f args args' :
-    OnOne2 (red1 Σ) args args' -> Σ ⊢ TApp f args ~> TApp f args'
+    OnOne2 (red1 flags Σ) args args' -> Σ ⊢ TApp f args ~>{flags} TApp f args'
 
-where "Σ ⊢ t ~> u" := (red1 Σ t u).
+where "Σ ⊢ t ~>{ f } u" := (red1 f Σ t u).
 
 Set Elimination Schemes.
 
 Derive Signature for red1.
+
+Notation "Σ ⊢ t ~> u" := (red1 red_flags_all Σ t u)
+  (at level 50, no associativity, t at next level, u at next level).
 
 (***********************************************************************)
 (** * Induction principle for [red1]. *)
@@ -60,41 +65,43 @@ Derive Signature for red1.
 
 (** Induction principle for [red1]. We can't use Rocq's default induction principle
     because [red1] is nested over [OnOne2]. *)
-Lemma red1_ind (P : forall s, evar_map -> term s -> term s -> Prop) :
-  (forall s Σ x ty body arg args,
-    P s Σ (TApp (TLam x ty body) (arg :: args)) (TApp (body[x := arg]) args)) ->
-  (forall s Σ ev ty def,
+Lemma red1_ind (flags : red_flags) (Σ : evar_map) (P : forall s, term s -> term s -> Prop) :
+  (forall s x ty body arg args,
+    flags.(beta) = true ->
+    P s (TApp (TLam x ty body) (arg :: args)) (TApp (body[x := arg]) args)) ->
+  (forall s ev ty def,
+    flags.(evars) = true ->
     Σ ev = Some (mk_evar_entry ty (Some def)) ->
-    P s Σ (TEvar ev) (wk def)) ->
-  (forall s Σ x ty ty' body,
-    Σ ⊢ ty ~> ty' ->
-    P s Σ ty ty' ->
-    P s Σ (TLam x ty body) (TLam x ty' body)) ->
-  (forall s Σ x ty body body',
-    Σ ⊢ body ~> body' ->
-    P (s ▷ x) Σ body body' ->
-    P s Σ (TLam x ty body) (TLam x ty body')) ->
-  (forall s Σ x a a' b,
-    Σ ⊢ a ~> a' ->
-    P s Σ a a' ->
-    P s Σ (TProd x a b) (TProd x a' b)) ->
-  (forall s Σ x a b b',
-    Σ ⊢ b ~> b' ->
-    P (s ▷ x) Σ b b' ->
-    P s Σ (TProd x a b) (TProd x a b')) ->
-  (forall s Σ f f' args,
-    Σ ⊢ f ~> f' ->
-    P s Σ f f' ->
-    P s Σ (TApp f args) (TApp f' args)) ->
-  (forall s Σ f args args',
-    OnOne2 (fun arg arg' => Σ ⊢ arg ~> arg' /\ P s Σ arg arg') args args' ->
-    P s Σ (TApp f args) (TApp f args')) ->
-  forall s Σ t t', Σ ⊢ t ~> t' -> P s Σ t t'.
+    P s (TEvar ev) (wk def)) ->
+  (forall s x ty ty' body,
+    Σ ⊢ ty ~>{flags} ty' ->
+    P s ty ty' ->
+    P s (TLam x ty body) (TLam x ty' body)) ->
+  (forall s x ty body body',
+    Σ ⊢ body ~>{flags} body' ->
+    P (s ▷ x) body body' ->
+    P s (TLam x ty body) (TLam x ty body')) ->
+  (forall s x a a' b,
+    Σ ⊢ a ~>{flags} a' ->
+    P s a a' ->
+    P s (TProd x a b) (TProd x a' b)) ->
+  (forall s x a b b',
+    Σ ⊢ b ~>{flags} b' ->
+    P (s ▷ x) b b' ->
+    P s (TProd x a b) (TProd x a b')) ->
+  (forall s f f' args,
+    Σ ⊢ f ~>{flags} f' ->
+    P s f f' ->
+    P s (TApp f args) (TApp f' args)) ->
+  (forall s f args args',
+    OnOne2 (fun arg arg' => Σ ⊢ arg ~>{flags} arg' /\ P s arg arg') args args' ->
+    P s (TApp f args) (TApp f args')) ->
+  forall s t t', Σ ⊢ t ~>{flags} t' -> P s t t'.
 Proof.
-intros Hbeta Hevar Hlam_l Hlam_r Hprod_l Hprod_r Happ_l Happ_r. fix IH 5.
-intros s Σ t t' Hred. destruct Hred.
-- apply Hbeta.
-- eapply Hevar. eassumption.
+intros Hbeta Hevar Hlam_l Hlam_r Hprod_l Hprod_r Happ_l Happ_r. fix IH 4.
+intros s t t' Hred. destruct Hred.
+- apply Hbeta ; auto.
+- eapply Hevar ; eauto.
 - apply Hlam_l ; auto.
 - apply Hlam_r ; auto.
 - apply Hprod_l ; auto.
@@ -109,76 +116,99 @@ Qed.
 (** * Reduction relation [red]. *)
 (***********************************************************************)
 
-Reserved Notation "Σ ⊢ t ~~> u"
+Reserved Notation "Σ ⊢ t ~~>{ f } u"
   (at level 50, no associativity, t at next level, u at next level).
 
 (** Strong reduction relation, defined as the reflexive-transitive closure of [red1]. *)
-Inductive red {s} (Σ : evar_map) : term s -> term s -> Prop :=
-| red_refl t : Σ ⊢ t ~~> t
-| red_step t1 t2 t3 : Σ ⊢ t1 ~~> t2 -> Σ ⊢ t2 ~> t3 -> Σ ⊢ t1 ~~> t3
+Inductive red (flags : red_flags) (Σ : evar_map) {s} : term s -> term s -> Prop :=
+| red_refl t : Σ ⊢ t ~~>{flags} t
+| red_step t1 t2 t3 : Σ ⊢ t1 ~~>{flags} t2 -> Σ ⊢ t2 ~>{flags} t3 -> Σ ⊢ t1 ~~>{flags} t3
 
-where  "Σ ⊢ t ~~> u" := (red Σ t u).
+where  "Σ ⊢ t ~~>{ f } u" := (red f Σ t u).
 
 Derive Signature for red.
 
-#[export] Instance red_Reflexive s Σ : Reflexive (@red s Σ).
+Notation "Σ ⊢ t ~~> u" := (red red_flags_all Σ t u)
+  (at level 50, no associativity, t at next level, u at next level).
+
+(***********************************************************************)
+(** * Typeclass instances for setoid rewriting. *)
+(***********************************************************************)
+
+#[export] Instance red_Reflexive flags Σ s : Reflexive (@red flags Σ s).
 Proof. intros t. apply red_refl. Qed.
 
-#[export] Instance red_Transitive s Σ : Transitive (@red s Σ).
+#[export] Instance red_Transitive flags Σ s : Transitive (@red flags Σ s).
 Proof.
 intros t1 t2 t3 H1 H2. induction H2.
 - assumption.
 - apply red_step with t2 ; auto.
 Qed.
 
-Lemma red_of_red1 {s} Σ (t u : term s) :
-  Σ ⊢ t ~> u -> Σ ⊢ t ~~> u.
+#[export] Instance red_of_red1 flags Σ s :
+  subrelation (@red1 flags Σ s) (@red flags Σ s).
+Proof. intros t u H. apply red_step with t ; auto. apply red_refl. Qed.
+
+Lemma red_same flags Σ {s} (t u : term s) :
+  t = u -> Σ ⊢ t ~~>{flags} u.
+Proof. intros ->. reflexivity. Qed.
+
+Lemma red1_extend_flags {flags1 flags2 Σ s} :
+  red_flags_incl flags1 flags2 ->
+  subrelation (@red1 flags1 Σ s) (@red1 flags2 Σ s).
 Proof.
-intros H. apply red_step with t ; auto. reflexivity.
+intros Hf t u Hred. induction Hred ; try now constructor.
+- constructor. now apply Hf.
+- econstructor ; [now apply Hf |]. eassumption.
+- constructor. revert H. apply OnOne2_consequence. firstorder.
 Qed.
 
-#[export] Instance subrelation_red1_red s Σ :
-  subrelation (@red1 s Σ) (@red s Σ).
-Proof. intros t u H. now apply red_of_red1. Qed.
-
-Lemma red_same {s} Σ (t u : term s) :
-  t = u -> Σ ⊢ t ~~> u.
-Proof. intros ->. reflexivity. Qed.
+Lemma red_extend_flags {flags1 flags2 Σ s} :
+  red_flags_incl flags1 flags2 ->
+  subrelation (@red flags1 Σ s) (@red flags2 Σ s).
+Proof.
+intros Hf t u Hred. induction Hred.
+- reflexivity.
+- transitivity t2.
+  + apply IHHred.
+  + apply (red1_extend_flags Hf) in H. now rewrite H.
+Qed.
 
 (***********************************************************************)
 (** * Congruence lemmas for [red1]. *)
 (***********************************************************************)
 
 Section CongruenceLemmas.
-  Context {s : scope} (Σ : evar_map).
+  Context (flags : red_flags) (Σ : evar_map) {s : scope}.
 
   Lemma red1_beta_alt x (ty : term s) body arg args t :
+    flags.(beta) = true ->
     t = TApp (body[x := arg]) args ->
-    Σ ⊢ TApp (TLam x ty body) (arg :: args) ~> t.
-  Proof. intros ->. apply red1_beta. Qed.
+    Σ ⊢ TApp (TLam x ty body) (arg :: args) ~>{flags} t.
+  Proof. intros H ->. now apply red1_beta. Qed.
 
   #[export] Instance red1_lam_congr_l x :
-    Proper (red1 Σ ==> eq ==> red1 Σ) (@TLam s x).
+    Proper (red1 flags Σ ==> eq ==> red1 flags Σ) (@TLam s x).
   Proof. intros ty ty' Hty body body' <-. now apply red1_lam_l. Qed.
 
   #[export] Instance red1_lam_congr_r x :
-    Proper (eq ==> red1 Σ ==> red1 Σ) (@TLam s x).
+    Proper (eq ==> red1 flags Σ ==> red1 flags Σ) (@TLam s x).
   Proof. intros ty ty' <- body body' Hbody. now apply red1_lam_r. Qed.
 
   #[export] Instance red1_prod_congr_l x :
-    Proper (red1 Σ ==> eq ==> red1 Σ) (@TProd s x).
+    Proper (red1 flags Σ ==> eq ==> red1 flags Σ) (@TProd s x).
   Proof. intros ty ty' Hty body body' <-. now apply red1_prod_l. Qed.
 
   #[export] Instance red1_prod_congr_r x :
-    Proper (eq ==> red1 Σ ==> red1 Σ) (@TProd s x).
+    Proper (eq ==> red1 flags Σ ==> red1 flags Σ) (@TProd s x).
   Proof. intros ty ty' <- body body' Hbody. now apply red1_prod_r. Qed.
 
   #[export] Instance red1_app_congr_l :
-    Proper (red1 Σ ==> eq ==> red1 Σ) (@TApp s).
+    Proper (red1 flags Σ ==> eq ==> red1 flags Σ) (@TApp s).
   Proof. intros f f' Hf args args' <-. now apply red1_app_l. Qed.
 
   #[export] Instance red1_app_congr_r :
-    Proper (eq ==> OnOne2 (red1 Σ) ==> red1 Σ) (@TApp s).
+    Proper (eq ==> OnOne2 (red1 flags Σ) ==> red1 flags Σ) (@TApp s).
   Proof. intros f f' <- args args' Hargs. now apply red1_app_r. Qed.
 
 End CongruenceLemmas.
@@ -188,24 +218,21 @@ End CongruenceLemmas.
 (***********************************************************************)
 
 Section CongruenceLemmas.
-  Context {s : scope} (Σ : evar_map).
-
-  Lemma red_beta_alt x (ty : term s) body arg args t :
-    t = TApp (body[x := arg]) args ->
-    Σ ⊢ TApp (TLam x ty body) (arg :: args) ~~> t.
-  Proof. intros ->. apply red_of_red1, red1_beta. Qed.
+  Context (flags : red_flags) (Σ : evar_map) {s : scope}.
 
   Lemma red_beta x (ty : term s) body arg args :
-    Σ ⊢ TApp (TLam x ty body) (arg :: args) ~~> TApp (body[x := arg]) args.
-  Proof. now rewrite red1_beta. Qed.
+    flags.(beta) = true ->
+    Σ ⊢ TApp (TLam x ty body) (arg :: args) ~~>{flags} TApp (body[x := arg]) args.
+  Proof. intros H. now rewrite red1_beta. Qed.
 
   Lemma red_evar_expand ev ty def :
+    flags.(evars) = true ->
     Σ ev = Some (mk_evar_entry ty (Some def)) ->
-    Σ ⊢ @TEvar s ev ~~> wk def.
-  Proof. intros H. rewrite red1_evar_expand ; eauto. reflexivity. Qed.
+    Σ ⊢ @TEvar s ev ~~>{flags} wk def.
+  Proof. intros H1 H2. rewrite red1_evar_expand ; eauto. reflexivity. Qed.
 
   #[export] Instance red_lam_congr x :
-    Proper (red Σ ==> red Σ ==> red Σ) (@TLam s x).
+    Proper (red flags Σ ==> red flags Σ ==> red flags Σ) (@TLam s x).
   Proof.
   intros ty ty' Hty body body' Hbody. transitivity (TLam x ty body').
   - clear Hty. induction Hbody.
@@ -217,7 +244,7 @@ Section CongruenceLemmas.
   Qed.
 
   #[export] Instance red_prod_congr x :
-    Proper (red Σ ==> red Σ ==> red Σ) (@TProd s x).
+    Proper (red flags Σ ==> red flags Σ ==> red flags Σ) (@TProd s x).
   Proof.
   intros a a' Ha b b' Hb. transitivity (TProd x a b').
   - clear Ha. induction Hb.
@@ -229,8 +256,8 @@ Section CongruenceLemmas.
   Qed.
 
   Lemma red_app_congr_aux (f : term s) l (args args' : list (term s)) :
-    All2 (red Σ) args args' ->
-    Σ ⊢ TApp f (l ++ args) ~~> TApp f (l ++ args').
+    All2 (red flags Σ) args args' ->
+    Σ ⊢ TApp f (l ++ args) ~~>{flags} TApp f (l ++ args').
   Proof.
   intros H. revert f l. depind H ; intros f l.
   - reflexivity.
@@ -243,7 +270,7 @@ Section CongruenceLemmas.
   Qed.
 
   #[export] Instance red_app_congr :
-    Proper (red Σ ==> All2 (red Σ) ==> red Σ) (@TApp s).
+    Proper (red flags Σ ==> All2 (red flags Σ) ==> red flags Σ) (@TApp s).
   Proof.
   intros f f' Hf args arg' Hargs. transitivity (TApp f' args).
   - clear Hargs. induction Hf.
@@ -259,10 +286,10 @@ End CongruenceLemmas.
 (***********************************************************************)
 
 Section InversionLemmas.
-  Context {s : scope} (Σ : evar_map).
+  Context (flags : red_flags) (Σ : evar_map) {s : scope}.
 
   Lemma red_type_inv (t : term s) :
-    Σ ⊢ TType ~~> t -> t = TType.
+    Σ ⊢ TType ~~>{flags} t -> t = TType.
   Proof.
   intros H. depind H.
   - reflexivity.
@@ -270,7 +297,7 @@ Section InversionLemmas.
   Qed.
 
   Lemma red_var_inv (i : index s) (t : term s) :
-    Σ ⊢ TVar i ~~> t -> t = TVar i.
+    Σ ⊢ TVar i ~~>{flags} t -> t = TVar i.
   Proof.
   intros H. depind H.
   - reflexivity.
@@ -278,11 +305,11 @@ Section InversionLemmas.
   Qed.
 
   Lemma red_lam_inv x (ty : term s) body t :
-    Σ ⊢ TLam x ty body ~~> t ->
+    Σ ⊢ TLam x ty body ~~>{flags} t ->
     exists ty' body',
       t = TLam x ty' body' /\
-      Σ ⊢ ty ~~> ty' /\
-      Σ ⊢ body ~~> body'.
+      Σ ⊢ ty ~~>{flags} ty' /\
+      Σ ⊢ body ~~>{flags} body'.
   Proof.
   intros Hred. depind Hred.
   - exists ty, body. now split3.
@@ -294,11 +321,11 @@ Section InversionLemmas.
   Qed.
 
   Lemma red_prod_inv x (a : term s) b t :
-    Σ ⊢ TProd x a b ~~> t ->
+    Σ ⊢ TProd x a b ~~>{flags} t ->
     exists a' b',
       t = TProd x a' b' /\
-      Σ ⊢ a ~~> a' /\
-      Σ ⊢ b ~~> b'.
+      Σ ⊢ a ~~>{flags} a' /\
+      Σ ⊢ b ~~>{flags} b'.
   Proof.
   intros Hred. depind Hred.
   - exists a, b. now split3.
