theories/MetaTheory/Reduction/RedFlags.v
@@ -1,0 +1,55 @@
+From Metaprog Require Import Prelude.
+
+(** This module defines _reduction flags_ which control which rules
+    are allowed in the various reduction & conversion relations
+    (e.g. [red] and [conv]).
+*)
+
+(***********************************************************************)
+(** * Reduction flags. *)
+(***********************************************************************)
+
+(** Reduction flags [red_flags] control which rules are allowed in reduction:
+    - [beta] controls beta reduction (function application).
+    - [evars] controls evar expansion. *)
+Record red_flags := {
+  beta : bool ;
+  evars : bool
+}.
+
+(** All reduction rules enabled. *)
+Definition red_flags_all : red_flags :=
+  {| beta := true ; evars := true |}.
+
+(** All reduction rules disabled. *)
+Definition red_flags_none : red_flags :=
+  {| beta := false ; evars := false |}.
+
+(** Only evar expansion is enabled. *)
+Definition red_flags_evars : red_flags :=
+  {| beta := false ; evars := true |}.
+
+(***********************************************************************)
+(** * Inclusion on reduction flags. *)
+(***********************************************************************)
+
+Record red_flags_incl (f1 f2 : red_flags) : Prop := {
+  red_flags_incl_beta : f1.(beta) = true -> f2.(beta) = true ;
+  red_flags_incl_evars : f1.(evars) = true -> f2.(evars) = true
+}.
+
+#[export] Instance red_flags_incl_Reflexive : Reflexive red_flags_incl.
+Proof. intros f. constructor ; auto. Qed.
+
+#[export] Instance red_flags_incl_Transitive : Transitive red_flags_incl.
+Proof.
+intros f1 f2 f3 H1 H2. constructor ; intros H ; now apply H1, H2 in H.
+Qed.
+
+Lemma red_flags_incl_none_l f :
+  red_flags_incl red_flags_none f.
+Proof. constructor ; cbn ; intros H ; depelim H. Qed.
+
+Lemma red_flags_incl_all_r f :
+  red_flags_incl f red_flags_all.
+Proof. constructor ; cbn ; auto. Qed.
